adding new optimization: reducing code size

tests/DxOpcode.v
@@ -9,215 +9,153 @@ Require Import CoqIntegers DxIntegers InfComp GenMatchable.
 
 Open Scope Z_scope.
 
-Inductive opcode_alu64_imm: Type := (**r 0xX7 *)
+Inductive opcode_alu64: Type := (**r 0xX7 *)
   (** ALU64:13 *)
-  | op_BPF_ADD64i
-  | op_BPF_SUB64i
-  | op_BPF_MUL64i
-  | op_BPF_DIV64i
-  | op_BPF_OR64i
-  | op_BPF_AND64i
-  | op_BPF_LSH64i
-  | op_BPF_RSH64i
+  | op_BPF_ADD64
+  | op_BPF_SUB64
+  | op_BPF_MUL64
+  | op_BPF_DIV64
+  | op_BPF_OR64
+  | op_BPF_AND64
+  | op_BPF_LSH64
+  | op_BPF_RSH64
   | op_BPF_NEG64
-  | op_BPF_MOD64i
-  | op_BPF_XOR64i
-  | op_BPF_MOV64i
-  | op_BPF_ARSH64i
-  | op_BPF_ALU64_IMM_ILLEGAL_INS.
+  | op_BPF_MOD64
+  | op_BPF_XOR64
+  | op_BPF_MOV64
+  | op_BPF_ARSH64
+  | op_BPF_ALU64_ILLEGAL_INS.
 
+(**
+#define BPF_INSTRUCTION_ALU_OP_MASK     0xf0
 
-Definition int64_to_opcode_alu64_imm (ins: int64_t): opcode_alu64_imm :=
-  let opcode := Int64.unsigned (Int64.and ins int64_0xff) in (**r masking operation *)
-    match opcode with
-    | 0x07 => op_BPF_ADD64i
-    | 0x17 => op_BPF_SUB64i
-    | 0x27 => op_BPF_MUL64i
-    | 0x37 => op_BPF_DIV64i
-    | 0x47 => op_BPF_OR64i
-    | 0x57 => op_BPF_AND64i
-    | 0x67 => op_BPF_LSH64i
-    | 0x77 => op_BPF_RSH64i
-    | 0x87 => op_BPF_NEG64
-    | 0x97 => op_BPF_MOD64i
-    | 0xa7 => op_BPF_XOR64i
-    | 0xb7 => op_BPF_MOV64i
-    | 0xc7 => op_BPF_ARSH64i
-    | _    => op_BPF_ALU64_IMM_ILLEGAL_INS
+#define BPF_INSTRUCTION_ALU_ADD         0x00
+#define BPF_INSTRUCTION_ALU_SUB         0x10
+#define BPF_INSTRUCTION_ALU_MUL         0x20
+#define BPF_INSTRUCTION_ALU_DIV         0x30
+#define BPF_INSTRUCTION_ALU_OR          0x40
+#define BPF_INSTRUCTION_ALU_AND         0x50
+#define BPF_INSTRUCTION_ALU_LSH         0x60
+#define BPF_INSTRUCTION_ALU_RSH         0x70
+#define BPF_INSTRUCTION_ALU_NEG         0x80
+#define BPF_INSTRUCTION_ALU_MOD         0x90
+#define BPF_INSTRUCTION_ALU_XOR         0xA0
+#define BPF_INSTRUCTION_ALU_MOV         0xB0
+#define BPF_INSTRUCTION_ALU_ARSH        0xC0
+
+*)
+
+Definition byte_to_opcode_alu64 (op: int8_t): opcode_alu64 :=
+  let opcode_alu := Byte.unsigned (Byte.and op int8_0xf0) in (**r masking operation *)
+    match opcode_alu with
+    | 0x00 => op_BPF_ADD64
+    | 0x10 => op_BPF_SUB64
+    | 0x20 => op_BPF_MUL64
+    | 0x30 => op_BPF_DIV64
+    | 0x40 => op_BPF_OR64
+    | 0x50 => op_BPF_AND64
+    | 0x60 => op_BPF_LSH64
+    | 0x70 => op_BPF_RSH64
+    | 0x80 => op_BPF_NEG64
+    | 0x90 => op_BPF_MOD64
+    | 0xa0 => op_BPF_XOR64
+    | 0xb0 => op_BPF_MOV64
+    | 0xc0 => op_BPF_ARSH64
+    | _    => op_BPF_ALU64_ILLEGAL_INS
     end.
 
-Inductive opcode_alu64_reg: Type := (**r 0xXf *)
-  (** ALU64:12 *)
-  | op_BPF_ADD64r
-  | op_BPF_SUB64r
-  | op_BPF_MUL64r
-  | op_BPF_DIV64r
-  | op_BPF_OR64r
-  | op_BPF_AND64r
-  | op_BPF_LSH64r
-  | op_BPF_RSH64r
-  | op_BPF_MOD64r
-  | op_BPF_XOR64r
-  | op_BPF_MOV64r
-  | op_BPF_ARSH64r
-  | op_BPF_ALU64_REG_ILLEGAL_INS.
-
-Definition int64_to_opcode_alu64_reg (ins: int64_t): opcode_alu64_reg :=
-  let opcode := Int64.unsigned (Int64.and ins int64_0xff) in (**r masking operation *)
-    match opcode with
-    | 0x0f => op_BPF_ADD64r
-    | 0x1f => op_BPF_SUB64r
-    | 0x2f => op_BPF_MUL64r
-    | 0x3f => op_BPF_DIV64r
-    | 0x4f => op_BPF_OR64r
-    | 0x5f => op_BPF_AND64r
-    | 0x6f => op_BPF_LSH64r
-    | 0x7f => op_BPF_RSH64r
-    | 0x9f => op_BPF_MOD64r
-    | 0xaf => op_BPF_XOR64r
-    | 0xbf => op_BPF_MOV64r
-    | 0xcf => op_BPF_ARSH64r
-    | _    => op_BPF_ALU64_REG_ILLEGAL_INS
-    end.
-
-Inductive opcode_alu32_imm: Type := (**r 0xX4 *)
+Inductive opcode_alu32: Type := (**r 0xX4 *)
   (** ALU32:13 *)
-  | op_BPF_ADD32i
-  | op_BPF_SUB32i
-  | op_BPF_MUL32i
-  | op_BPF_DIV32i
-  | op_BPF_OR32i
-  | op_BPF_AND32i
-  | op_BPF_LSH32i
-  | op_BPF_RSH32i
+  | op_BPF_ADD32
+  | op_BPF_SUB32
+  | op_BPF_MUL32
+  | op_BPF_DIV32
+  | op_BPF_OR32
+  | op_BPF_AND32
+  | op_BPF_LSH32
+  | op_BPF_RSH32
   | op_BPF_NEG32
-  | op_BPF_MOD32i
-  | op_BPF_XOR32i
-  | op_BPF_MOV32i
-  | op_BPF_ARSH32i
-  | op_BPF_ALU32_IMM_ILLEGAL_INS.
+  | op_BPF_MOD32
+  | op_BPF_XOR32
+  | op_BPF_MOV32
+  | op_BPF_ARSH32
+  | op_BPF_ALU32_ILLEGAL_INS.
 
-Definition int64_to_opcode_alu32_imm (ins: int64_t): opcode_alu32_imm :=
-  let opcode := Int64.unsigned (Int64.and ins int64_0xff) in (**r masking operation *)
-    match opcode with
-    | 0x04 => op_BPF_ADD32i
-    | 0x14 => op_BPF_SUB32i
-    | 0x24 => op_BPF_MUL32i
-    | 0x34 => op_BPF_DIV32i
-    | 0x44 => op_BPF_OR32i
-    | 0x54 => op_BPF_AND32i
-    | 0x64 => op_BPF_LSH32i
-    | 0x74 => op_BPF_RSH32i
-    | 0x84 => op_BPF_NEG32
-    | 0x94 => op_BPF_MOD32i
-    | 0xa4 => op_BPF_XOR32i
-    | 0xb4 => op_BPF_MOV32i
-    | 0xc4 => op_BPF_ARSH32i
-    | _    => op_BPF_ALU32_IMM_ILLEGAL_INS
+
+Definition byte_to_opcode_alu32 (op: int8_t): opcode_alu32 :=
+  let opcode_alu := Byte.unsigned (Byte.and op int8_0xf0) in (**r masking operation *)
+    match opcode_alu with
+    | 0x00 => op_BPF_ADD32
+    | 0x10 => op_BPF_SUB32
+    | 0x20 => op_BPF_MUL32
+    | 0x30 => op_BPF_DIV32
+    | 0x40 => op_BPF_OR32
+    | 0x50 => op_BPF_AND32
+    | 0x60 => op_BPF_LSH32
+    | 0x70 => op_BPF_RSH32
+    | 0x80 => op_BPF_NEG32
+    | 0x90 => op_BPF_MOD32
+    | 0xa0 => op_BPF_XOR32
+    | 0xb0 => op_BPF_MOV32
+    | 0xc0 => op_BPF_ARSH32
+    | _    => op_BPF_ALU32_ILLEGAL_INS
     end.
 
-Inductive opcode_alu32_reg: Type := (**r 0xXc *)
-  (** ALU32:12 *)
-  | op_BPF_ADD32r
-  | op_BPF_SUB32r
-  | op_BPF_MUL32r
-  | op_BPF_DIV32r
-  | op_BPF_OR32r
-  | op_BPF_AND32r
-  | op_BPF_LSH32r
-  | op_BPF_RSH32r
-  | op_BPF_MOD32r
-  | op_BPF_XOR32r
-  | op_BPF_MOV32r
-  | op_BPF_ARSH32r
-  | op_BPF_ALU32_REG_ILLEGAL_INS.
-
-Definition int64_to_opcode_alu32_reg (ins: int64_t): opcode_alu32_reg :=
-  let opcode := Int64.unsigned (Int64.and ins int64_0xff) in (**r masking operation *)
-    match opcode with
-    | 0x0c => op_BPF_ADD32r
-    | 0x1c => op_BPF_SUB32r
-    | 0x2c => op_BPF_MUL32r
-    | 0x3c => op_BPF_DIV32r
-    | 0x4c => op_BPF_OR32r
-    | 0x5c => op_BPF_AND32r
-    | 0x6c => op_BPF_LSH32r
-    | 0x7c => op_BPF_RSH32r
-    | 0x9c => op_BPF_MOD32r
-    | 0xac => op_BPF_XOR32r
-    | 0xbc => op_BPF_MOV32r
-    | 0xcc => op_BPF_ARSH32r
-    | _    => op_BPF_ALU32_REG_ILLEGAL_INS
-    end.
-
-Inductive opcode_branch_imm: Type := (**r 0xX5 *)
+Inductive opcode_branch: Type := (**r 0xX5 *)
   (**Branch: 13 *)
   | op_BPF_JA
-  | op_BPF_JEQi
-  | op_BPF_JGTi
-  | op_BPF_JGEi
-  | op_BPF_JLTi
-  | op_BPF_JLEi
-  | op_BPF_JSETi
-  | op_BPF_JNEi
-  | op_BPF_JSGTi
-  | op_BPF_JSGEi
-  | op_BPF_JSLTi
-  | op_BPF_JSLEi
+  | op_BPF_JEQ
+  | op_BPF_JGT
+  | op_BPF_JGE
+  | op_BPF_JLT
+  | op_BPF_JLE
+  | op_BPF_JSET
+  | op_BPF_JNE
+  | op_BPF_JSGT
+  | op_BPF_JSGE
+  | op_BPF_JSLT
+  | op_BPF_JSLE
   | op_BPF_RET
-  | op_BPF_JMP_IMM_ILLEGAL_INS.
+  | op_BPF_JMP_ILLEGAL_INS.
 
-Definition int64_to_opcode_branch_imm (ins: int64_t): opcode_branch_imm :=
-  let opcode := Int64.unsigned (Int64.and ins int64_0xff) in (**r masking operation *)
-    match opcode with
-    | 0x05 => op_BPF_JA
-    | 0x15 => op_BPF_JEQi
-    | 0x25 => op_BPF_JGTi
-    | 0x35 => op_BPF_JGEi
-    | 0xa5 => op_BPF_JLTi
-    | 0xb5 => op_BPF_JLEi
-    | 0x45 => op_BPF_JSETi
-    | 0x55 => op_BPF_JNEi
-    | 0x65 => op_BPF_JSGTi
-    | 0x75 => op_BPF_JSGEi
-    | 0xc5 => op_BPF_JSLTi
-    | 0xd5 => op_BPF_JSLEi
+(**
+#define BPF_INSTRUCTION_ALU_OP_MASK     0xf0
+
+#define BPF_INSTRUCTION_BRANCH_JA       0x00
+#define BPF_INSTRUCTION_BRANCH_JEQ      0x10
+#define BPF_INSTRUCTION_BRANCH_JGT      0x20
+#define BPF_INSTRUCTION_BRANCH_JGE      0x30
+#define BPF_INSTRUCTION_BRANCH_JLT      0xa0
+#define BPF_INSTRUCTION_BRANCH_JLE      0xb0
+#define BPF_INSTRUCTION_BRANCH_JSET     0x40
+#define BPF_INSTRUCTION_BRANCH_JNE      0x50
+#define BPF_INSTRUCTION_BRANCH_JSGT     0x60
+#define BPF_INSTRUCTION_BRANCH_JSGE     0x70
+#define BPF_INSTRUCTION_BRANCH_JSLT     0xc0
+#define BPF_INSTRUCTION_BRANCH_JSLE     0xd0
+#define BPF_INSTRUCTION_BRANCH_CALL     0x80
+#define BPF_INSTRUCTION_BRANCH_EXIT     0x90
+*)
+
+Definition byte_to_opcode_branch (op: int8_t): opcode_branch :=
+  let opcode_jmp := Byte.unsigned (Byte.and op int8_0xf0) in (**r masking operation *)
+    match opcode_jmp with
+    | 0x00 => op_BPF_JA
+    | 0x10 => op_BPF_JEQ
+    | 0x20 => op_BPF_JGT
+    | 0x30 => op_BPF_JGE
+    | 0xa0 => op_BPF_JLT
+    | 0xb0 => op_BPF_JLE
+    | 0x40 => op_BPF_JSET
+    | 0x50 => op_BPF_JNE
+    | 0x60 => op_BPF_JSGT
+    | 0x70 => op_BPF_JSGE
+    | 0xc0 => op_BPF_JSLT
+    | 0xd0 => op_BPF_JSLE
   (*
     | 0x85 => op_BPF_CALL*)
-    | 0x95 => op_BPF_RET
-    | _    => op_BPF_JMP_IMM_ILLEGAL_INS
-    end.
-
-Inductive opcode_branch_reg: Type := (**r 0xXd *)
-  (**Branch: 11 *)
-  | op_BPF_JEQr
-  | op_BPF_JGTr
-  | op_BPF_JGEr
-  | op_BPF_JLTr
-  | op_BPF_JLEr
-  | op_BPF_JSETr
-  | op_BPF_JNEr
-  | op_BPF_JSGTr
-  | op_BPF_JSGEr
-  | op_BPF_JSLTr
-  | op_BPF_JSLEr
-  | op_BPF_JMP_REG_ILLEGAL_INS.
-
-Definition int64_to_opcode_branch_reg (ins: int64_t): opcode_branch_reg :=
-  let opcode := Int64.unsigned (Int64.and ins int64_0xff) in (**r masking operation *)
-    match opcode with
-    | 0x1d => op_BPF_JEQr
-    | 0x2d => op_BPF_JGTr
-    | 0x3d => op_BPF_JGEr
-    | 0xad => op_BPF_JLTr
-    | 0xbd => op_BPF_JLEr
-    | 0x4d => op_BPF_JSETr
-    | 0x5d => op_BPF_JNEr
-    | 0x6d => op_BPF_JSGTr
-    | 0x7d => op_BPF_JSGEr
-    | 0xcd => op_BPF_JSLTr
-    | 0xdd => op_BPF_JSLEr
-    | _    => op_BPF_JMP_REG_ILLEGAL_INS
+    | 0x90 => op_BPF_RET
+    | _    => op_BPF_JMP_ILLEGAL_INS
     end.
 
 Inductive opcode_mem_ld_imm: Type :=  (**r 0xX8 *)
@@ -225,9 +163,9 @@ Inductive opcode_mem_ld_imm: Type :=  (**r 0xX8 *)
   | op_BPF_LDDW
   | op_BPF_LDX_IMM_ILLEGAL_INS.
 
-Definition int64_to_opcode_mem_ld_imm (ins: int64_t): opcode_mem_ld_imm :=
-  let opcode := Int64.unsigned (Int64.and ins int64_0xff) in (**r masking operation *)
-    match opcode with
+Definition byte_to_opcode_mem_ld_imm (op: int8_t): opcode_mem_ld_imm :=
+  let opcode_ld := Byte.unsigned (Byte.and op int8_0xff) in (**r masking operation *)
+    match opcode_ld with
     | 0x18 => op_BPF_LDDW
     | _    => op_BPF_LDX_IMM_ILLEGAL_INS
     end.
@@ -240,9 +178,9 @@ Inductive opcode_mem_ld_reg: Type :=  (**r 0xX1/0xX9 *)
   | op_BPF_LDXDW
   | op_BPF_LDX_REG_ILLEGAL_INS.
 
-Definition int64_to_opcode_mem_ld_reg (ins: int64_t): opcode_mem_ld_reg :=
-  let opcode := Int64.unsigned (Int64.and ins int64_0xff) in (**r masking operation *)
-    match opcode with
+Definition byte_to_opcode_mem_ld_reg (op: int8_t): opcode_mem_ld_reg :=
+  let opcode_ld := Byte.unsigned (Byte.and op int8_0xff) in (**r masking operation *)
+    match opcode_ld with
     | 0x61 => op_BPF_LDXW
     | 0x69 => op_BPF_LDXH
     | 0x71 => op_BPF_LDXB
@@ -257,9 +195,9 @@ Inductive opcode_mem_st_imm: Type :=  (**r 0xX2/0xXa *)
   | op_BPF_STDW
   | op_BPF_ST_ILLEGAL_INS.
 
-Definition int64_to_opcode_mem_st_imm (ins: int64_t): opcode_mem_st_imm :=
-  let opcode := Int64.unsigned (Int64.and ins int64_0xff) in (**r masking operation *)
-    match opcode with
+Definition byte_to_opcode_mem_st_imm (op: int8_t): opcode_mem_st_imm :=
+  let opcode_st := Byte.unsigned (Byte.and op int8_0xff) in (**r masking operation *)
+    match opcode_st with
     | 0x62 => op_BPF_STW
     | 0x6a => op_BPF_STH
     | 0x72 => op_BPF_STB
@@ -274,9 +212,9 @@ Inductive opcode_mem_st_reg: Type :=  (**r 0xX3/0xXb *)
   | op_BPF_STXDW
   | op_BPF_STX_ILLEGAL_INS.
 
-Definition int64_to_opcode_mem_st_reg (ins: int64_t): opcode_mem_st_reg :=
-  let opcode := Int64.unsigned (Int64.and ins int64_0xff) in (**r masking operation *)
-    match opcode with
+Definition byte_to_opcode_mem_st_reg (op: int8_t): opcode_mem_st_reg :=
+  let opcode_st := Byte.unsigned (Byte.and op int8_0xff) in (**r masking operation *)
+    match opcode_st with
     | 0x63 => op_BPF_STXW
     | 0x6b => op_BPF_STXH
     | 0x73 => op_BPF_STXB
@@ -285,12 +223,9 @@ Definition int64_to_opcode_mem_st_reg (ins: int64_t): opcode_mem_st_reg :=
     end.
 
 Inductive opcode: Type :=
-  | op_BPF_ALU64_imm   (**r 0xX7 *)
-  | op_BPF_ALU64_reg   (**r 0xXf *)
-  | op_BPF_ALU32_imm   (**r 0xX4 *)
-  | op_BPF_ALU32_reg   (**r 0xXc *)
-  | op_BPF_Branch_imm  (**r 0xX5 *)
-  | op_BPF_Branch_reg  (**r 0xXd *)
+  | op_BPF_ALU64   (**r 0xX7 / 0xXf *)
+  | op_BPF_ALU32   (**r 0xX4 / 0xXc *)
+  | op_BPF_Branch  (**r 0xX5 / 0xXd *)
   | op_BPF_Mem_ld_imm  (**r 0xX8 *)
   | op_BPF_Mem_ld_reg  (**r 0xX1/0xX9 *)
   | op_BPF_Mem_st_imm  (**r 0xX2/0xXa *)
@@ -298,148 +233,87 @@ Inductive opcode: Type :=
 
   | op_BPF_ILLEGAL_INS.
 
-Definition int64_to_opcode (ins: int64_t): opcode :=
-  let opcode := Int64.unsigned (Int64.and ins int64_0xf) in (**r masking operation *)
-    match opcode with
-    | 0x07 => op_BPF_ALU64_imm
-    | 0x0f => op_BPF_ALU64_reg
-    | 0x04 => op_BPF_ALU32_imm
-    | 0x0c => op_BPF_ALU32_reg
-    | 0x05 => op_BPF_Branch_imm
-    | 0x0d => op_BPF_Branch_reg
-    | 0x08 => op_BPF_Mem_ld_imm
+(**
+#define BPF_INSTRUCTION_CLS_MASK        0x07
+
+#define BPF_INSTRUCTION_CLS_LD          0x00
+#define BPF_INSTRUCTION_CLS_LDX         0x01
+#define BPF_INSTRUCTION_CLS_ST          0x02
+#define BPF_INSTRUCTION_CLS_STX         0x03
+#define BPF_INSTRUCTION_CLS_ALU32       0x04
+#define BPF_INSTRUCTION_CLS_BRANCH      0x05
+#define BPF_INSTRUCTION_CLS_ALU64       0x07
+*)
+Definition byte_to_opcode (op: int8_t): opcode :=
+  let opc := Byte.unsigned (Byte.and op int8_0x07) in (**r masking operation *)
+    match opc with
+    | 0x07 => op_BPF_ALU64
+    | 0x04 => op_BPF_ALU32
+    | 0x05 => op_BPF_Branch
+    | 0x00 => op_BPF_Mem_ld_imm
     | 0x01 => op_BPF_Mem_ld_reg
-    | 0x09 => op_BPF_Mem_ld_reg
     | 0x02 => op_BPF_Mem_st_imm
-    | 0x0a => op_BPF_Mem_st_imm
     | 0x03 => op_BPF_Mem_st_reg
-    | 0x0b => op_BPF_Mem_st_reg
     | _    => op_BPF_ILLEGAL_INS
     end.
-(*
-Inductive opcode: Type :=
-  | op_BPF_ALU64_imm : opcode_alu64_imm  -> opcode  (**r 0xX7 *)
-  | op_BPF_ALU64_reg : opcode_alu64_reg  -> opcode  (**r 0xXf *)
-  | op_BPF_ALU32_imm : opcode_alu32_imm  -> opcode  (**r 0xX4 *)
-  | op_BPF_ALU32_reg : opcode_alu32_reg  -> opcode  (**r 0xXc *)
-  | op_BPF_Branch_imm: opcode_branch_imm -> opcode  (**r 0xX5 *)
-  | op_BPF_Branch_reg: opcode_branch_reg -> opcode  (**r 0xXd *)
-  | op_BPF_Mem_ld_imm: opcode_mem_ld_imm -> opcode  (**r 0xX8 *)
-  | op_BPF_Mem_ld_reg: opcode_mem_ld_reg -> opcode  (**r 0xX1/0xX9 *)
-  | op_BPF_Mem_st_imm: opcode_mem_st_imm -> opcode  (**r 0xX2/0xXa *)
-  | op_BPF_Mem_st_reg: opcode_mem_st_reg -> opcode  (**r 0xX3/0xXb *)
 
-  | op_BPF_ILLEGAL_INS. *)
-
+Definition int64_to_opcode (ins: int64_t): int8_t := Byte.repr (Int64.unsigned (Int64.and ins int64_0xff)).
 
 (******************** Dx related *******************)
 
-Definition opcode_alu64_imm_eqb  (o o' : opcode_alu64_imm): bool :=
+Definition opcode_alu64_eqb  (o o' : opcode_alu64): bool :=
   match o , o' with
-  | op_BPF_ADD64i, op_BPF_ADD64i
-  | op_BPF_SUB64i, op_BPF_SUB64i
-  | op_BPF_MUL64i, op_BPF_MUL64i
-  | op_BPF_DIV64i, op_BPF_DIV64i
-  | op_BPF_OR64i,  op_BPF_OR64i
-  | op_BPF_AND64i, op_BPF_AND64i
-  | op_BPF_LSH64i, op_BPF_LSH64i
-  | op_BPF_RSH64i, op_BPF_RSH64i
+  | op_BPF_ADD64, op_BPF_ADD64
+  | op_BPF_SUB64, op_BPF_SUB64
+  | op_BPF_MUL64, op_BPF_MUL64
+  | op_BPF_DIV64, op_BPF_DIV64
+  | op_BPF_OR64,  op_BPF_OR64
+  | op_BPF_AND64, op_BPF_AND64
+  | op_BPF_LSH64, op_BPF_LSH64
+  | op_BPF_RSH64, op_BPF_RSH64
   | op_BPF_NEG64,  op_BPF_NEG64
-  | op_BPF_MOD64i, op_BPF_MOD64i
-  | op_BPF_XOR64i, op_BPF_XOR64i
-  | op_BPF_MOV64i, op_BPF_MOV64i
-  | op_BPF_ARSH64i,op_BPF_ARSH64i
-  | op_BPF_ALU64_IMM_ILLEGAL_INS, op_BPF_ALU64_IMM_ILLEGAL_INS => true
+  | op_BPF_MOD64, op_BPF_MOD64
+  | op_BPF_XOR64, op_BPF_XOR64
+  | op_BPF_MOV64, op_BPF_MOV64
+  | op_BPF_ARSH64,op_BPF_ARSH64
+  | op_BPF_ALU64_ILLEGAL_INS, op_BPF_ALU64_ILLEGAL_INS => true
   | _, _ => false
   end.
 
-Definition opcode_alu64_reg_eqb  (o o' : opcode_alu64_reg): bool :=
+Definition opcode_alu32_eqb  (o o' : opcode_alu32) : bool :=
   match o , o' with
-  | op_BPF_ADD64r, op_BPF_ADD64r
-  | op_BPF_SUB64r, op_BPF_SUB64r
-  | op_BPF_MUL64r, op_BPF_MUL64r
-  | op_BPF_DIV64r, op_BPF_DIV64r
-  | op_BPF_OR64r,  op_BPF_OR64r
-  | op_BPF_AND64r, op_BPF_AND64r
-  | op_BPF_LSH64r, op_BPF_LSH64r
-  | op_BPF_RSH64r, op_BPF_RSH64r
-  | op_BPF_MOD64r, op_BPF_MOD64r
-  | op_BPF_XOR64r, op_BPF_XOR64r
-  | op_BPF_MOV64r, op_BPF_MOV64r
-  | op_BPF_ARSH64r,op_BPF_ARSH64r
-  | op_BPF_ALU64_REG_ILLEGAL_INS, op_BPF_ALU64_REG_ILLEGAL_INS => true
-  | _, _ => false
-  end.
-
-Definition opcode_alu32_imm_eqb  (o o' : opcode_alu32_imm) : bool :=
-  match o , o' with
-  | op_BPF_ADD32i, op_BPF_ADD32i
-  | op_BPF_SUB32i, op_BPF_SUB32i
-  | op_BPF_MUL32i, op_BPF_MUL32i
-  | op_BPF_DIV32i, op_BPF_DIV32i
-  | op_BPF_OR32i,  op_BPF_OR32i
-  | op_BPF_AND32i, op_BPF_AND32i
-  | op_BPF_LSH32i, op_BPF_LSH32i
-  | op_BPF_RSH32i, op_BPF_RSH32i
+  | op_BPF_ADD32, op_BPF_ADD32
+  | op_BPF_SUB32, op_BPF_SUB32
+  | op_BPF_MUL32, op_BPF_MUL32
+  | op_BPF_DIV32, op_BPF_DIV32
+  | op_BPF_OR32,  op_BPF_OR32
+  | op_BPF_AND32, op_BPF_AND32
+  | op_BPF_LSH32, op_BPF_LSH32
+  | op_BPF_RSH32, op_BPF_RSH32
   | op_BPF_NEG32,  op_BPF_NEG32
-  | op_BPF_MOD32i, op_BPF_MOD32i
-  | op_BPF_XOR32i, op_BPF_XOR32i
-  | op_BPF_MOV32i, op_BPF_MOV32i
-  | op_BPF_ALU32_IMM_ILLEGAL_INS, op_BPF_ALU32_IMM_ILLEGAL_INS => true
+  | op_BPF_MOD32, op_BPF_MOD32
+  | op_BPF_XOR32, op_BPF_XOR32
+  | op_BPF_MOV32, op_BPF_MOV32
+  | op_BPF_ALU32_ILLEGAL_INS, op_BPF_ALU32_ILLEGAL_INS => true
   | _, _ => false
   end.
 
-Definition opcode_alu32_reg_eqb  (o o' : opcode_alu32_reg) : bool :=
+Definition opcode_branch_eqb (o o' : opcode_branch): bool :=
   match o , o' with
-  | op_BPF_ADD32r, op_BPF_ADD32r
-  | op_BPF_SUB32r, op_BPF_SUB32r
-  | op_BPF_MUL32r, op_BPF_MUL32r
-  | op_BPF_DIV32r, op_BPF_DIV32r
-  | op_BPF_OR32r,  op_BPF_OR32r
-  | op_BPF_AND32r, op_BPF_AND32r
-  | op_BPF_LSH32r, op_BPF_LSH32r
-  | op_BPF_RSH32r, op_BPF_RSH32r
-  | op_BPF_MOD32r, op_BPF_MOD32r
-  | op_BPF_XOR32r, op_BPF_XOR32r
-  | op_BPF_MOV32r, op_BPF_MOV32r
-  | op_BPF_ARSH32r,op_BPF_ARSH32r
-  | op_BPF_ALU32_REG_ILLEGAL_INS, op_BPF_ALU32_REG_ILLEGAL_INS => true
-  | _, _ => false
-  end.
-
-Definition opcode_branch_imm_eqb (o o' : opcode_branch_imm): bool :=
-  match o , o' with
-  | op_BPF_JA,     op_BPF_JA
-  | op_BPF_JEQi,   op_BPF_JEQi
-  | op_BPF_JGTi,   op_BPF_JGTi
-  | op_BPF_JGEi,   op_BPF_JGEi
-  | op_BPF_JLTi,   op_BPF_JLTi
-  | op_BPF_JLEi,   op_BPF_JLEi
-  | op_BPF_JSETi,  op_BPF_JSETi
-  | op_BPF_JNEi,   op_BPF_JNEi
-  | op_BPF_JSGTi,  op_BPF_JSGTi
-  | op_BPF_JSGEi,  op_BPF_JSGEi
-  | op_BPF_JSLTi,  op_BPF_JSLTi
-  | op_BPF_JSLEi,  op_BPF_JSLEi
-  | op_BPF_RET,    op_BPF_RET
-  | op_BPF_JMP_IMM_ILLEGAL_INS, op_BPF_JMP_IMM_ILLEGAL_INS => true
-  | _, _ => false
-  end.
-
-Definition opcode_branch_reg_eqb (o o' : opcode_branch_reg): bool :=
-  match o , o' with
-  | op_BPF_JEQr,   op_BPF_JEQr
-  | op_BPF_JGTr,   op_BPF_JGTr
-  | op_BPF_JGEr,   op_BPF_JGEr
-  | op_BPF_JLTr,   op_BPF_JLTr
-  | op_BPF_JLEr,   op_BPF_JLEr
-  | op_BPF_JSETr,  op_BPF_JSETr
-  | op_BPF_JNEr,   op_BPF_JNEr
-  | op_BPF_JSGTr,  op_BPF_JSGTr
-  | op_BPF_JSGEr,  op_BPF_JSGEr
-  | op_BPF_JSLTr,  op_BPF_JSLTr
-  | op_BPF_JSLEr,  op_BPF_JSLEr
-  | op_BPF_JMP_REG_ILLEGAL_INS, op_BPF_JMP_REG_ILLEGAL_INS => true
+  | op_BPF_JA,    op_BPF_JA
+  | op_BPF_JEQ,   op_BPF_JEQ
+  | op_BPF_JGT,   op_BPF_JGT
+  | op_BPF_JGE,   op_BPF_JGE
+  | op_BPF_JLT,   op_BPF_JLT
+  | op_BPF_JLE,   op_BPF_JLE
+  | op_BPF_JSET,  op_BPF_JSET
+  | op_BPF_JNE,   op_BPF_JNE
+  | op_BPF_JSGT,  op_BPF_JSGT
+  | op_BPF_JSGE,  op_BPF_JSGE
+  | op_BPF_JSLT,  op_BPF_JSLT
+  | op_BPF_JSLE,  op_BPF_JSLE
+  | op_BPF_RET,   op_BPF_RET
+  | op_BPF_JMP_ILLEGAL_INS, op_BPF_JMP_ILLEGAL_INS => true
   | _, _ => false
   end.
 
@@ -482,12 +356,9 @@ Definition opcode_mem_st_reg_eqb (o o' : opcode_mem_st_reg): bool :=
 
 Definition opcode_eqb (o o' : opcode) : bool :=
   match o , o' with
-  | op_BPF_ALU64_imm , op_BPF_ALU64_imm
-  | op_BPF_ALU64_reg , op_BPF_ALU64_reg
-  | op_BPF_ALU32_imm , op_BPF_ALU32_imm
-  | op_BPF_ALU32_reg , op_BPF_ALU32_reg
-  | op_BPF_Branch_imm, op_BPF_Branch_imm
-  | op_BPF_Branch_reg, op_BPF_Branch_reg
+  | op_BPF_ALU64,      op_BPF_ALU64
+  | op_BPF_ALU32,      op_BPF_ALU32
+  | op_BPF_Branch,     op_BPF_Branch
   | op_BPF_Mem_ld_imm, op_BPF_Mem_ld_imm
   | op_BPF_Mem_ld_reg, op_BPF_Mem_ld_reg
   | op_BPF_Mem_st_imm, op_BPF_Mem_st_imm
@@ -498,140 +369,75 @@ Definition opcode_eqb (o o' : opcode) : bool :=
   end.
 
 
-Definition opcode_alu64_immCompilableType :=
-  MkCompilableType opcode_alu64_imm C_U8.
+Definition opcode_alu64CompilableType :=
+  MkCompilableType opcode_alu64 C_U8.
 
-Definition opcode_alu64_immCompilableTypeMatchableType : MatchableType:=
+Definition opcode_alu64CompilableTypeMatchableType : MatchableType:=
   Eval compute in
  (mkEnumMatchableType
-    opcode_alu64_immCompilableType  opcode_alu64_imm_eqb
-    (     (op_BPF_ADD64i, 0x07)
-       :: (op_BPF_SUB64i, 0x17)
-       :: (op_BPF_MUL64i, 0x27)
-       :: (op_BPF_DIV64i, 0x37)
-       :: (op_BPF_OR64i,  0x47)
-       :: (op_BPF_AND64i, 0x57)
-       :: (op_BPF_LSH64i, 0x67)
-       :: (op_BPF_RSH64i, 0x77)
-       :: (op_BPF_NEG64,  0x87)
-       :: (op_BPF_MOD64i, 0x97)
-       :: (op_BPF_XOR64i, 0xa7)
-       :: (op_BPF_MOV64i, 0xb7)
-       :: (op_BPF_ARSH64i,0xc7):: nil)
-    op_BPF_ALU64_IMM_ILLEGAL_INS
-    (fun m A => opcode_alu64_imm_rect (fun _ => m A))).
+    opcode_alu64CompilableType  opcode_alu64_eqb
+    (     (op_BPF_ADD64, 0x00)
+       :: (op_BPF_SUB64, 0x10)
+       :: (op_BPF_MUL64, 0x20)
+       :: (op_BPF_DIV64, 0x30)
+       :: (op_BPF_OR64,  0x40)
+       :: (op_BPF_AND64, 0x50)
+       :: (op_BPF_LSH64, 0x60)
+       :: (op_BPF_RSH64, 0x70)
+       :: (op_BPF_NEG64, 0x80)
+       :: (op_BPF_MOD64, 0x90)
+       :: (op_BPF_XOR64, 0xa0)
+       :: (op_BPF_MOV64, 0xb0)
+       :: (op_BPF_ARSH64,0xc0):: nil)
+    op_BPF_ALU64_ILLEGAL_INS
+    (fun m A => opcode_alu64_rect (fun _ => m A))).
 
-Definition opcode_alu64_regCompilableType :=
-  MkCompilableType opcode_alu64_reg C_U8.
+Definition opcode_alu32CompilableType :=
+  MkCompilableType opcode_alu32 C_U8.
 
-Definition opcode_alu64_regCompilableTypeMatchableType : MatchableType:=
+Definition opcode_alu32CompilableTypeMatchableType : MatchableType:=
   Eval compute in
  (mkEnumMatchableType
-    opcode_alu64_regCompilableType  opcode_alu64_reg_eqb
-    (     (op_BPF_ADD64r, 0x0f)
-       :: (op_BPF_SUB64r, 0x1f)
-       :: (op_BPF_MUL64r, 0x2f)
-       :: (op_BPF_DIV64r, 0x3f)
-       :: (op_BPF_OR64r,  0x4f)
-       :: (op_BPF_AND64r, 0x5f)
-       :: (op_BPF_LSH64r, 0x6f)
-       :: (op_BPF_RSH64r, 0x7f)
-       :: (op_BPF_MOD64r, 0x9f)
-       :: (op_BPF_XOR64r, 0xaf)
-       :: (op_BPF_MOV64r, 0xbf)
-       :: (op_BPF_ARSH64r,0xcf):: nil)
-    op_BPF_ALU64_REG_ILLEGAL_INS
-    (fun m A => opcode_alu64_reg_rect (fun _ => m A))).
+    opcode_alu32CompilableType  opcode_alu32_eqb
+    (     (op_BPF_ADD32, 0x00)
+       :: (op_BPF_SUB32, 0x10)
+       :: (op_BPF_MUL32, 0x20)
+       :: (op_BPF_DIV32, 0x30)
+       :: (op_BPF_OR32,  0x40)
+       :: (op_BPF_AND32, 0x50)
+       :: (op_BPF_LSH32, 0x60)
+       :: (op_BPF_RSH32, 0x70)
+       :: (op_BPF_NEG32, 0x80)
+       :: (op_BPF_MOD32, 0x90)
+       :: (op_BPF_XOR32, 0xa0)
+       :: (op_BPF_MOV32, 0xb0)
+       :: (op_BPF_ARSH32,0xc0) :: nil)
+    op_BPF_ALU32_ILLEGAL_INS
+    (fun m A => opcode_alu32_rect (fun _ => m A))).
 
-Definition opcode_alu32_immCompilableType :=
-  MkCompilableType opcode_alu32_imm C_U8.
+Definition opcode_branchCompilableType :=
+  MkCompilableType opcode_branch C_U8.
 
-Definition opcode_alu32_immCompilableTypeMatchableType : MatchableType:=
+Definition opcode_branchCompilableTypeMatchableType : MatchableType:=
   Eval compute in
  (mkEnumMatchableType
-    opcode_alu32_immCompilableType  opcode_alu32_imm_eqb
-    (     (op_BPF_ADD32i, 0x04)
-       :: (op_BPF_SUB32i, 0x14)
-       :: (op_BPF_MUL32i, 0x24)
-       :: (op_BPF_DIV32i, 0x34)
-       :: (op_BPF_OR32i,  0x44)
-       :: (op_BPF_AND32i, 0x54)
-       :: (op_BPF_LSH32i, 0x64)
-       :: (op_BPF_RSH32i, 0x74)
-       :: (op_BPF_NEG32,  0x84)
-       :: (op_BPF_MOD32i, 0x94)
-       :: (op_BPF_XOR32i, 0xa4)
-       :: (op_BPF_MOV32i, 0xb4)
-       :: (op_BPF_ARSH32i,0xc4) :: nil)
-    op_BPF_ALU32_IMM_ILLEGAL_INS
-    (fun m A => opcode_alu32_imm_rect (fun _ => m A))).
+    opcode_branchCompilableType  opcode_branch_eqb
+    (     (op_BPF_JA,   0x00)
+       :: (op_BPF_JEQ,  0x10)
+       :: (op_BPF_JGT,  0x20)
+       :: (op_BPF_JGE,  0x30)
+       :: (op_BPF_JSET, 0x40)
+       :: (op_BPF_JNE,  0x50)
+       :: (op_BPF_JSGT, 0x60)
+       :: (op_BPF_JSGE, 0x70)
 
-Definition opcode_alu32_regCompilableType :=
-  MkCompilableType opcode_alu32_reg C_U8.
-
-Definition opcode_alu32_regCompilableTypeMatchableType : MatchableType:=
-  Eval compute in
- (mkEnumMatchableType
-    opcode_alu32_regCompilableType  opcode_alu32_reg_eqb
-    (     (op_BPF_ADD32r, 0x0c)
-       :: (op_BPF_SUB32r, 0x1c)
-       :: (op_BPF_MUL32r, 0x2c)
-       :: (op_BPF_DIV32r, 0x3c)
-       :: (op_BPF_OR32r,  0x4c)
-       :: (op_BPF_AND32r, 0x5c)
-       :: (op_BPF_LSH32r, 0x6c)
-       :: (op_BPF_RSH32r, 0x7c)
-       :: (op_BPF_MOD32r, 0x9c)
-       :: (op_BPF_XOR32r, 0xac)
-       :: (op_BPF_MOV32r, 0xbc)
-       :: (op_BPF_ARSH32r,0xcc) :: nil)
-    op_BPF_ALU32_REG_ILLEGAL_INS
-    (fun m A => opcode_alu32_reg_rect (fun _ => m A))).
-
-Definition opcode_branch_immCompilableType :=
-  MkCompilableType opcode_branch_imm C_U8.
-
-Definition opcode_branch_immCompilableTypeMatchableType : MatchableType:=
-  Eval compute in
- (mkEnumMatchableType
-    opcode_branch_immCompilableType  opcode_branch_imm_eqb
-    (     (op_BPF_JA,   0x05)
-       :: (op_BPF_JEQi, 0x15)
-       :: (op_BPF_JGTi, 0x25)
-       :: (op_BPF_JGEi, 0x35)
-       :: (op_BPF_JSETi,0x45)
-       :: (op_BPF_JNEi, 0x55)
-       :: (op_BPF_JSGTi,0x65)
-       :: (op_BPF_JSGEi,0x75)
-
-       :: (op_BPF_RET,  0x95)
-       :: (op_BPF_JLTi, 0xa5)
-       :: (op_BPF_JLEi, 0xb5)
-       :: (op_BPF_JSLTi,0xc5)
-       :: (op_BPF_JSLEi, 0xd5) :: nil)
-    op_BPF_JMP_IMM_ILLEGAL_INS
-    (fun m A => opcode_branch_imm_rect (fun _ => m A))).
-
-Definition opcode_branch_regCompilableType :=
-  MkCompilableType opcode_branch_reg C_U8.
-
-Definition opcode_branch_regCompilableTypeMatchableType : MatchableType:=
-  Eval compute in
- (mkEnumMatchableType
-    opcode_branch_regCompilableType  opcode_branch_reg_eqb
-    (     (op_BPF_JEQr, 0x1d)
-       :: (op_BPF_JGTr, 0x2d)
-       :: (op_BPF_JGEr, 0x3d)
-       :: (op_BPF_JLTr, 0xad)
-       :: (op_BPF_JLEr, 0xbd)
-       :: (op_BPF_JSETr,0x4d)
-       :: (op_BPF_JNEr, 0x5d)
-       :: (op_BPF_JSGTr,0x6d)
-       :: (op_BPF_JSGEr,0x7d)
-       :: (op_BPF_JSLTr,0xcd)
-       :: (op_BPF_JSLEr,0xdd) :: nil)
-    op_BPF_JMP_REG_ILLEGAL_INS
-    (fun m A => opcode_branch_reg_rect (fun _ => m A))).
+       :: (op_BPF_RET,  0x90)
+       :: (op_BPF_JLT,  0xa0)
+       :: (op_BPF_JLE,  0xb0)
+       :: (op_BPF_JSLT, 0xc0)
+       :: (op_BPF_JSLE, 0xd0) :: nil)
+    op_BPF_JMP_ILLEGAL_INS
+    (fun m A => opcode_branch_rect (fun _ => m A))).
 
 Definition opcode_mem_ld_immCompilableType :=
   MkCompilableType opcode_mem_ld_imm C_U8.
@@ -690,204 +496,149 @@ Definition opcode_mem_st_regCompilableTypeMatchableType : MatchableType:=
 Definition opcodeCompilableType :=
   MkCompilableType opcode C_U8.
 
-Definition opcodeMatchableType :=
-  MkMatchableType opcodeCompilableType
-    (fun x cases =>
-      match cases with
-      | [r0; r1; r2; r3; r4; r5; r6; r7; r8; r9; r10] =>
-        Ok (Csyntax.Sswitch x
-              (Csyntax.LScons (Some 0x07) r0
-                (Csyntax.LScons (Some 0x0f) r1
-                  (Csyntax.LScons (Some 0x04) r2
-                    (Csyntax.LScons (Some 0x0c) r3
-                      (Csyntax.LScons (Some 0x05) r4
-                        (Csyntax.LScons (Some 0x0d) r5
-                          (Csyntax.LScons (Some 0x08) r6
-                            (Csyntax.LScons (Some 0x01) r7
-                              (Csyntax.LScons (Some 0x09) r7
-                                (Csyntax.LScons (Some 0x02) r8
-                                  (Csyntax.LScons (Some 0x0a) r8
-                                    (Csyntax.LScons (Some 0x03) r9
-                                      (Csyntax.LScons (Some 0x0b) r9
-                                        (Csyntax.LScons None r10
-                                          Csyntax.LSnil))))))))))))))
-            )
-      | _ => Err MatchEncodingFailed
-      end)
-    [[]; []; []; []; []; []; []; []; []; []; []]
-    [[]; []; []; []; []; []; []; []; []; []; []]
-    (fun m A r whenR0 whenR1 whenR2 whenR3 whenR4 whenR5 whenR6 whenR7 whenR8 whenR9 whenR10 =>
-      match r with
-      | op_BPF_ALU64_imm => whenR0
-      | op_BPF_ALU64_reg => whenR1
-      | op_BPF_ALU32_imm => whenR2
-      | op_BPF_ALU32_reg => whenR3
-      | op_BPF_Branch_imm => whenR4
-      | op_BPF_Branch_reg => whenR5
-      | op_BPF_Mem_ld_imm => whenR6
-      | op_BPF_Mem_ld_reg => whenR7
-      | op_BPF_Mem_st_imm => whenR8
-      | op_BPF_Mem_st_reg => whenR9
-      | op_BPF_ILLEGAL_INS => whenR10
-      end).
+Definition opcodeCompilableTypeMatchableType : MatchableType:=
+  Eval compute in
+ (mkEnumMatchableType
+    opcodeCompilableType  opcode_eqb
+    (     (op_BPF_ALU64,      0x07)
+       :: (op_BPF_ALU32,      0x04)
+       :: (op_BPF_Branch,     0x05)
+       :: (op_BPF_Mem_ld_imm, 0x00)
+       :: (op_BPF_Mem_ld_reg, 0x01)
+       :: (op_BPF_Mem_st_imm, 0x02)
+       :: (op_BPF_Mem_st_reg, 0x03):: nil)
+    op_BPF_ILLEGAL_INS
+    (fun m A => opcode_rect (fun _ => m A))).
+
+
+Definition byteToopcodeSymbolType :=
+  MkCompilableSymbolType [int8CompilableType] (Some opcodeCompilableType).
 
 Definition int64ToopcodeSymbolType :=
   MkCompilableSymbolType [int64CompilableType] (Some opcodeCompilableType).
 
 
-Instance CINT : CType int64_t := mkCType _ (cType int64CompilableType).
+Instance CINT : CType int8_t := mkCType _ (cType int8CompilableType).
 Instance COP : CType opcode := mkCType _ (cType opcodeCompilableType).
+Instance CINT64 : CType int64_t := mkCType _ (cType int64CompilableType).
 
 Definition Const_int64_to_opcode :=
   ltac: (mkprimitive int64_to_opcode
                 (fun es => match es with
-                           | [e1] => Ok (Csyntax.Ecast (Csyntax.Ebinop Cop.Oand e1 C_U64_0xf C_U64) C_U8)
-                           | _       => Err PrimitiveEncodingFailed
-                           end)).
-
-Definition int64_to_opcode_alu64_immSymbolType :=
-  MkCompilableSymbolType [int64CompilableType] (Some opcode_alu64_immCompilableType).
-
-Instance COP_alu64_imm : CType opcode_alu64_imm := mkCType _ (cType opcode_alu64_immCompilableType).
-
-Definition Const_int64_to_opcode_alu64_imm :=
-  ltac: (mkprimitive int64_to_opcode_alu64_imm
-                (fun es => match es with
                            | [e1] => Ok (Csyntax.Ecast (Csyntax.Ebinop Cop.Oand e1 C_U64_0xff C_U64) C_U8)
                            | _       => Err PrimitiveEncodingFailed
                            end)).
 
-Definition int64_to_opcode_alu64_regSymbolType :=
-  MkCompilableSymbolType [int64CompilableType] (Some opcode_alu64_regCompilableType).
 
-Instance COP_alu64_reg : CType opcode_alu64_reg := mkCType _ (cType opcode_alu64_regCompilableType).
-
-Definition Const_int64_to_opcode_alu64_reg :=
-  ltac: (mkprimitive int64_to_opcode_alu64_reg
+Definition Const_byte_to_opcode :=
+  ltac: (mkprimitive byte_to_opcode
                 (fun es => match es with
-                           | [e1] => Ok (Csyntax.Ecast (Csyntax.Ebinop Cop.Oand e1 C_U64_0xff C_U64) C_U8)
+                           | [e1] => Ok (Csyntax.Ecast (Csyntax.Ebinop Cop.Oand e1 C_U8_0x07 C_U8) C_U8)
                            | _       => Err PrimitiveEncodingFailed
                            end)).
 
-Definition int64_to_opcode_alu32_immSymbolType :=
-  MkCompilableSymbolType [int64CompilableType] (Some opcode_alu32_immCompilableType).
+Definition byte_to_opcode_alu64SymbolType :=
+  MkCompilableSymbolType [int8CompilableType] (Some opcode_alu64CompilableType).
 
-Instance COP_alu32_imm : CType opcode_alu32_imm := mkCType _ (cType opcode_alu32_immCompilableType).
+Instance COP_alu64 : CType opcode_alu64 := mkCType _ (cType opcode_alu64CompilableType).
 
-Definition Const_int64_to_opcode_alu32_imm :=
-  ltac: (mkprimitive int64_to_opcode_alu32_imm
+Definition Const_byte_to_opcode_alu64 :=
+  ltac: (mkprimitive byte_to_opcode_alu64
                 (fun es => match es with
-                           | [e1] => Ok (Csyntax.Ecast (Csyntax.Ebinop Cop.Oand e1 C_U64_0xff C_U64) C_U8)
+                           | [e1] => Ok (Csyntax.Ecast (Csyntax.Ebinop Cop.Oand e1 C_U8_0xf0 C_U8) C_U8)
                            | _       => Err PrimitiveEncodingFailed
                            end)).
 
-Definition int64_to_opcode_alu32_regSymbolType :=
-  MkCompilableSymbolType [int64CompilableType] (Some opcode_alu32_regCompilableType).
+Definition byte_to_opcode_alu32SymbolType :=
+  MkCompilableSymbolType [int8CompilableType] (Some opcode_alu32CompilableType).
 
-Instance COP_alu32_reg : CType opcode_alu32_reg := mkCType _ (cType opcode_alu32_regCompilableType).
+Instance COP_alu32 : CType opcode_alu32 := mkCType _ (cType opcode_alu32CompilableType).
 
-Definition Const_int64_to_opcode_alu32_reg :=
-  ltac: (mkprimitive int64_to_opcode_alu32_reg
+Definition Const_byte_to_opcode_alu32 :=
+  ltac: (mkprimitive byte_to_opcode_alu32
                 (fun es => match es with
-                           | [e1] => Ok (Csyntax.Ecast (Csyntax.Ebinop Cop.Oand e1 C_U64_0xff C_U64) C_U8)
+                           | [e1] => Ok (Csyntax.Ecast (Csyntax.Ebinop Cop.Oand e1 C_U8_0xf0 C_U8) C_U8)
                            | _       => Err PrimitiveEncodingFailed
                            end)).
 
-Definition int64_to_opcode_branch_immSymbolType :=
-  MkCompilableSymbolType [int64CompilableType] (Some opcode_branch_immCompilableType).
+Definition byte_to_opcode_branchSymbolType :=
+  MkCompilableSymbolType [int8CompilableType] (Some opcode_branchCompilableType).
 
-Instance COP_opcode_branch_imm : CType opcode_branch_imm := mkCType _ (cType opcode_branch_immCompilableType).
+Instance COP_opcode_branch : CType opcode_branch := mkCType _ (cType opcode_branchCompilableType).
 
-Definition Const_int64_to_opcode_branch_imm :=
-  ltac: (mkprimitive int64_to_opcode_branch_imm
+Definition Const_byte_to_opcode_branch :=
+  ltac: (mkprimitive byte_to_opcode_branch
                 (fun es => match es with
-                           | [e1] => Ok (Csyntax.Ecast (Csyntax.Ebinop Cop.Oand e1 C_U64_0xff C_U64) C_U8)
+                           | [e1] => Ok (Csyntax.Ecast (Csyntax.Ebinop Cop.Oand e1 C_U8_0xf0 C_U8) C_U8)
                            | _       => Err PrimitiveEncodingFailed
                            end)).
 
-Definition int64_to_opcode_branch_regSymbolType :=
-  MkCompilableSymbolType [int64CompilableType] (Some opcode_branch_regCompilableType).
-
-Instance COP_opcode_branch_reg : CType opcode_branch_reg := mkCType _ (cType opcode_branch_regCompilableType).
-
-Definition Const_int64_to_opcode_branch_reg :=
-  ltac: (mkprimitive int64_to_opcode_branch_reg
-                (fun es => match es with
-                           | [e1] => Ok (Csyntax.Ecast (Csyntax.Ebinop Cop.Oand e1 C_U64_0xff C_U64) C_U8)
-                           | _       => Err PrimitiveEncodingFailed
-                           end)).
-
-Definition int64_to_opcode_mem_ld_immSymbolType :=
-  MkCompilableSymbolType [int64CompilableType] (Some opcode_mem_ld_immCompilableType).
+Definition byte_to_opcode_mem_ld_immSymbolType :=
+  MkCompilableSymbolType [int8CompilableType] (Some opcode_mem_ld_immCompilableType).
 
 Instance COP_opcode_mem_ld_imm : CType opcode_mem_ld_imm := mkCType _ (cType opcode_mem_ld_immCompilableType).
 
-Definition Const_int64_to_opcode_mem_ld_imm :=
-  ltac: (mkprimitive int64_to_opcode_mem_ld_imm
+Definition Const_byte_to_opcode_mem_ld_imm :=
+  ltac: (mkprimitive byte_to_opcode_mem_ld_imm
                 (fun es => match es with
-                           | [e1] => Ok (Csyntax.Ecast (Csyntax.Ebinop Cop.Oand e1 C_U64_0xff C_U64) C_U8)
+                           | [e1] => Ok (Csyntax.Ecast (Csyntax.Ebinop Cop.Oand e1 C_U8_0xff C_U8) C_U8)
                            | _       => Err PrimitiveEncodingFailed
                            end)).
 
-Definition int64_to_opcode_mem_ld_regSymbolType :=
-  MkCompilableSymbolType [int64CompilableType] (Some opcode_mem_ld_regCompilableType).
+Definition byte_to_opcode_mem_ld_regSymbolType :=
+  MkCompilableSymbolType [int8CompilableType] (Some opcode_mem_ld_regCompilableType).
 
 Instance COP_opcode_mem_ld_reg : CType opcode_mem_ld_reg := mkCType _ (cType opcode_mem_ld_regCompilableType).
 
-Definition Const_int64_to_opcode_mem_ld_reg :=
-  ltac: (mkprimitive int64_to_opcode_mem_ld_reg
+Definition Const_byte_to_opcode_mem_ld_reg :=
+  ltac: (mkprimitive byte_to_opcode_mem_ld_reg
                 (fun es => match es with
-                           | [e1] => Ok (Csyntax.Ecast (Csyntax.Ebinop Cop.Oand e1 C_U64_0xff C_U64) C_U8)
+                           | [e1] => Ok (Csyntax.Ecast (Csyntax.Ebinop Cop.Oand e1 C_U8_0xff C_U8) C_U8)
                            | _       => Err PrimitiveEncodingFailed
                            end)).
 
-Definition int64_to_opcode_mem_st_immSymbolType :=
-  MkCompilableSymbolType [int64CompilableType] (Some opcode_mem_st_immCompilableType).
+Definition byte_to_opcode_mem_st_immSymbolType :=
+  MkCompilableSymbolType [int8CompilableType] (Some opcode_mem_st_immCompilableType).
 
 Instance COP_opcode_mem_st_imm : CType opcode_mem_st_imm := mkCType _ (cType opcode_mem_st_immCompilableType).
 
-Definition Const_int64_to_opcode_mem_st_imm :=
-  ltac: (mkprimitive int64_to_opcode_mem_st_imm
+Definition Const_byte_to_opcode_mem_st_imm :=
+  ltac: (mkprimitive byte_to_opcode_mem_st_imm
                 (fun es => match es with
-                           | [e1] => Ok (Csyntax.Ecast (Csyntax.Ebinop Cop.Oand e1 C_U64_0xff C_U64) C_U8)
+                           | [e1] => Ok (Csyntax.Ecast (Csyntax.Ebinop Cop.Oand e1 C_U8_0xff C_U8) C_U8)
                            | _       => Err PrimitiveEncodingFailed
                            end)).
 
-Definition int64_to_opcode_mem_st_regSymbolType :=
-  MkCompilableSymbolType [int64CompilableType] (Some opcode_mem_st_regCompilableType).
+Definition byte_to_opcode_mem_st_regSymbolType :=
+  MkCompilableSymbolType [int8CompilableType] (Some opcode_mem_st_regCompilableType).
 
 Instance COP_opcode_mem_st_reg : CType opcode_mem_st_reg := mkCType _ (cType opcode_mem_st_regCompilableType).
 
-Definition Const_int64_to_opcode_mem_st_reg :=
-  ltac: (mkprimitive int64_to_opcode_mem_st_reg
+Definition Const_byte_to_opcode_mem_st_reg :=
+  ltac: (mkprimitive byte_to_opcode_mem_st_reg
                 (fun es => match es with
-                           | [e1] => Ok (Csyntax.Ecast (Csyntax.Ebinop Cop.Oand e1 C_U64_0xff C_U64) C_U8)
+                           | [e1] => Ok (Csyntax.Ecast (Csyntax.Ebinop Cop.Oand e1 C_U8_0xff C_U8) C_U8)
                            | _       => Err PrimitiveEncodingFailed
                            end)).
 
 Close Scope Z_scope.
 
 Module Exports.
-  Definition opcode_alu64_immCompilableTypeMatchableType  := opcode_alu64_immCompilableTypeMatchableType.
-  Definition opcode_alu64_regCompilableTypeMatchableType  := opcode_alu64_regCompilableTypeMatchableType.
-  Definition opcode_alu32_immCompilableTypeMatchableType  := opcode_alu32_immCompilableTypeMatchableType.
-  Definition opcode_alu32_regCompilableTypeMatchableType  := opcode_alu32_regCompilableTypeMatchableType.
-  Definition opcode_branch_immCompilableTypeMatchableType := opcode_branch_immCompilableTypeMatchableType.
-  Definition opcode_branch_regCompilableTypeMatchableType := opcode_branch_regCompilableTypeMatchableType.
+  Definition opcode_alu64CompilableTypeMatchableType      := opcode_alu64CompilableTypeMatchableType.
+  Definition opcode_alu32CompilableTypeMatchableType      := opcode_alu32CompilableTypeMatchableType.
+  Definition opcode_branchCompilableTypeMatchableType     := opcode_branchCompilableTypeMatchableType.
   Definition opcode_mem_ld_immCompilableTypeMatchableType := opcode_mem_ld_immCompilableTypeMatchableType.
   Definition opcode_mem_ld_regCompilableTypeMatchableType := opcode_mem_ld_regCompilableTypeMatchableType.
   Definition opcode_mem_st_immCompilableTypeMatchableType := opcode_mem_st_immCompilableTypeMatchableType.
   Definition opcode_mem_st_regCompilableTypeMatchableType := opcode_mem_st_regCompilableTypeMatchableType.
-  Definition opcodeMatchableType             := opcodeMatchableType.
-  Definition Const_int64_to_opcode_alu64_imm := Const_int64_to_opcode_alu64_imm.
-  Definition Const_int64_to_opcode_alu64_reg := Const_int64_to_opcode_alu64_reg.
-  Definition Const_int64_to_opcode_alu32_imm := Const_int64_to_opcode_alu32_imm.
-  Definition Const_int64_to_opcode_alu32_reg := Const_int64_to_opcode_alu32_reg.
-  Definition Const_int64_to_opcode_branch_imm:= Const_int64_to_opcode_branch_imm.
-  Definition Const_int64_to_opcode_branch_reg:= Const_int64_to_opcode_branch_reg.
-  Definition Const_int64_to_opcode_mem_ld_imm:= Const_int64_to_opcode_mem_ld_imm.
-  Definition Const_int64_to_opcode_mem_ld_reg:= Const_int64_to_opcode_mem_ld_reg.
-  Definition Const_int64_to_opcode_mem_st_imm:= Const_int64_to_opcode_mem_st_imm.
-  Definition Const_int64_to_opcode_mem_st_reg:= Const_int64_to_opcode_mem_st_reg.
-  Definition Const_int64_to_opcode           := Const_int64_to_opcode.
+  Definition opcodeCompilableTypeMatchableType            := opcodeCompilableTypeMatchableType.
+  Definition Const_byte_to_opcode_alu64                   := Const_byte_to_opcode_alu64.
+  Definition Const_byte_to_opcode_alu32                   := Const_byte_to_opcode_alu32.
+  Definition Const_byte_to_opcode_branch                  := Const_byte_to_opcode_branch.
+  Definition Const_byte_to_opcode_mem_ld_imm              := Const_byte_to_opcode_mem_ld_imm.
+  Definition Const_byte_to_opcode_mem_ld_reg              := Const_byte_to_opcode_mem_ld_reg.
+  Definition Const_byte_to_opcode_mem_st_imm              := Const_byte_to_opcode_mem_st_imm.
+  Definition Const_byte_to_opcode_mem_st_reg              := Const_byte_to_opcode_mem_st_reg.
+  Definition Const_byte_to_opcode                         := Const_byte_to_opcode.
+  Definition Const_int64_to_opcode                        := Const_int64_to_opcode.
 End Exports.
