tests/DxInstructions.v
@@ -69,47 +69,41 @@ Definition reg64_to_reg32 (d: val64_t): M valu32_t := returnM (val_intuoflongu d
 Definition get_src (ins: int64_t): M reg :=
   returnM (int64_to_src_reg ins).
 
-Definition get_offset (i:int64_t ):M int64_t := returnM (Int64.shru (Int64.shl i int64_32) int64_48).
+Definition get_offset (ins:int64_t ):M int64_t := returnM (Int64.shru (Int64.shl ins int64_32) int64_48).
 (** get_immediate: int64_t -> vals32_t. Tthe return type is vals32_t instead of sint32_t because `imm` is always used to be calculted with other `val` type.
   *)
-Definition eval_offset (i:int64_t ):M val64_t := returnM (int64_to_vlong i).
+Definition eval_offset (ins:int64_t ):M val64_t := returnM (int64_to_vlong ins).
 
-Definition get_immediate (i:int64_t):M sint32_t := returnM (int64_to_sint32 (Int64.shru i int64_32)).
+Definition get_immediate (ins:int64_t):M sint32_t := returnM (int64_to_sint32 (Int64.shru ins int64_32)).
 
-Definition eval_immediate (i: sint32_t): M val64_t := returnM ((Val.longofintu (sint32_to_vint i))).
+Definition eval_immediate (ins: sint32_t): M val64_t := returnM ((Val.longofintu (sint32_to_vint ins))).
 
-Definition get_opcode_alu64_imm (ins: int64_t): M opcode_alu64_imm :=
-  returnM (int64_to_opcode_alu64_imm ins).
-
-Definition get_opcode_alu64_reg (ins: int64_t): M opcode_alu64_reg :=
-  returnM (int64_to_opcode_alu64_reg ins).
-
-Definition get_opcode_alu32_imm (ins: int64_t): M opcode_alu32_imm :=
-  returnM (int64_to_opcode_alu32_imm ins).
-
-Definition get_opcode_alu32_reg (ins: int64_t): M opcode_alu32_reg :=
-  returnM (int64_to_opcode_alu32_reg ins).
-
-Definition get_opcode_branch_imm (ins: int64_t): M opcode_branch_imm :=
-  returnM (int64_to_opcode_branch_imm ins).
-
-Definition get_opcode_branch_reg (ins: int64_t): M opcode_branch_reg :=
-  returnM (int64_to_opcode_branch_reg ins).
-
-Definition get_opcode_mem_ld_imm (ins: int64_t): M opcode_mem_ld_imm :=
-  returnM (int64_to_opcode_mem_ld_imm ins).
-
-Definition get_opcode_mem_ld_reg (ins: int64_t): M opcode_mem_ld_reg :=
-  returnM (int64_to_opcode_mem_ld_reg ins).
-
-Definition get_opcode_mem_st_imm (ins: int64_t): M opcode_mem_st_imm :=
-  returnM (int64_to_opcode_mem_st_imm ins).
-
-Definition get_opcode_mem_st_reg (ins: int64_t): M opcode_mem_st_reg :=
-  returnM (int64_to_opcode_mem_st_reg ins).
-
-Definition get_opcode (ins: int64_t): M opcode :=
+Definition get_opcode_ins (ins: int64_t): M int8_t :=
   returnM (int64_to_opcode ins).
+
+Definition get_opcode_alu64 (op: int8_t): M opcode_alu64 :=
+  returnM (byte_to_opcode_alu64 op).
+
+Definition get_opcode_alu32 (op: int8_t): M opcode_alu32 :=
+  returnM (byte_to_opcode_alu32 op).
+
+Definition get_opcode_branch (op: int8_t): M opcode_branch :=
+  returnM (byte_to_opcode_branch op).
+
+Definition get_opcode_mem_ld_imm (op: int8_t): M opcode_mem_ld_imm :=
+  returnM (byte_to_opcode_mem_ld_imm op).
+
+Definition get_opcode_mem_ld_reg (op: int8_t): M opcode_mem_ld_reg :=
+  returnM (byte_to_opcode_mem_ld_reg op).
+
+Definition get_opcode_mem_st_imm (op: int8_t): M opcode_mem_st_imm :=
+  returnM (byte_to_opcode_mem_st_imm op).
+
+Definition get_opcode_mem_st_reg (op: int8_t): M opcode_mem_st_reg :=
+  returnM (byte_to_opcode_mem_st_reg op).
+
+Definition get_opcode (op: int8_t): M opcode :=
+  returnM (byte_to_opcode op).
 
 Definition get_addl (x y: val64_t): M val64_t := returnM (Val.addl x y).
 
@@ -127,24 +121,24 @@ Definition getMemRegion_start_addr (mr: memory_region): M val64_t := returnM (st
 
 Definition getMemRegion_block_size (mr: memory_region): M val64_t := returnM (block_size mr).
 
-Definition is_well_chunk_bool (chunk0: memory_chunk) : M bool :=
-  match chunk0 with
+Definition is_well_chunk_bool (chunk: memory_chunk) : M bool :=
+  match chunk with
   | Mint8unsigned | Mint16unsigned | Mint32 | Mint64 => returnM true
   | _ => returnM false
   end.
 
 
-Definition check_mem_aux (mr3: memory_region) (addr0: val64_t) (chunk1: memory_chunk): M val64_t :=
-  do well_chunk <- is_well_chunk_bool chunk1;
+Definition check_mem_aux (mr: memory_region) (addr: val64_t) (chunk: memory_chunk): M val64_t :=
+  do well_chunk <- is_well_chunk_bool chunk;
     if well_chunk then
-      do ptr <- getMemRegion_block_ptr mr3;
-      do start <- getMemRegion_start_addr mr3;
-      do size <- getMemRegion_block_size mr3;
-      do lo_ofs <- get_subl addr0 start;
-      do hi_ofs <- get_addl lo_ofs (memory_chunk_to_val64 chunk1);
+      do ptr <- getMemRegion_block_ptr mr;
+      do start <- getMemRegion_start_addr mr;
+      do size <- getMemRegion_block_size mr;
+      do lo_ofs <- get_subl addr start;
+      do hi_ofs <- get_addl lo_ofs (memory_chunk_to_val64 chunk);
         if (andb (complu_le val64_zero lo_ofs) (complu_lt hi_ofs size)) then
-          if (andb (complu_le lo_ofs (memory_chunk_to_val64_upbound chunk1))
-                   (compl_eq val64_zero (val64_modlu lo_ofs (memory_chunk_to_val64 chunk1)))) then
+          if (andb (complu_le lo_ofs (memory_chunk_to_val64_upbound chunk))
+                   (compl_eq val64_zero (val64_modlu lo_ofs (memory_chunk_to_val64 chunk)))) then
             returnM (Val.addl ptr lo_ofs) (**r > 0 *)
           else
             returnM val64_zero (**r = 0 *)
@@ -153,13 +147,13 @@ Definition check_mem_aux (mr3: memory_region) (addr0: val64_t) (chunk1: memory_c
     else
       returnM val64_zero.
 
-Definition check_mem (l: MyListType) (addr1: val64_t) (chunk2: memory_chunk) : M val64_t :=
+Definition check_mem (l: MyListType) (addr: val64_t) (chunk: memory_chunk) : M val64_t :=
   do mrs           <- eval_mem_regions;
-  do check_mem_ctx <- check_mem_aux (bpf_ctx mrs) addr1 chunk2;
+  do check_mem_ctx <- check_mem_aux (bpf_ctx mrs) addr chunk;
     if compl_eq check_mem_ctx val64_zero then
-      do check_mem_stk <- check_mem_aux (bpf_stk mrs) addr1 chunk2;
+      do check_mem_stk <- check_mem_aux (bpf_stk mrs) addr chunk;
         if compl_eq check_mem_stk val64_zero then
-          do check_mem_content <- check_mem_aux (content mrs) addr1 chunk2;
+          do check_mem_content <- check_mem_aux (content mrs) addr chunk;
           if compl_eq check_mem_content val64_zero then
             returnM val64_zero
           else
@@ -169,442 +163,215 @@ Definition check_mem (l: MyListType) (addr1: val64_t) (chunk2: memory_chunk) : M
     else
       returnM check_mem_ctx.
 
-Definition step_opcode_alu64_imm (l: MyListType): M unit :=
-  do pc     <- eval_pc;
-  do ins    <- list_get l pc;
-  do dst    <- get_dst ins;
-  do dst64  <- eval_reg dst;
-  do imm    <- get_immediate ins;
-  do imm64  <- eval_immediate imm;
-  do opcode <- get_opcode_alu64_imm ins;
-  match opcode with
-  | op_BPF_ADD64i   =>
-    do _ <- upd_reg dst (Val.addl    dst64 imm64);
-      upd_flag BPF_OK
-  | op_BPF_SUB64i   =>
-    do _ <- upd_reg dst (Val.subl    dst64 imm64);
-      upd_flag BPF_OK
-  | op_BPF_MUL64i   =>
-    do _ <- upd_reg dst (Val.mull    dst64 imm64);
-      upd_flag BPF_OK
-  | op_BPF_DIV64i   =>
-    if compl_ne imm64 val64_zero then
-      do _ <- upd_reg dst (val64_divlu dst64 imm64);
-        upd_flag BPF_OK
-    else
-      upd_flag BPF_ILLEGAL_DIV
-  | op_BPF_OR64i    =>
-    do _ <- upd_reg dst (Val.orl     dst64 imm64);
-        upd_flag BPF_OK
-  | op_BPF_AND64i   =>
-    do _ <- upd_reg dst (Val.andl    dst64 imm64);
-        upd_flag BPF_OK
-  | op_BPF_LSH64i   =>
-    if complu_lt imm64 val64_64 then (**r Int64.iwordsize' = int64_64 *)
-      do _ <- upd_reg dst (Val.shll    dst64 (sint32_to_vint imm)); (**r it may have problem with proof because of the implicitly type casting, let's see *)
-        upd_flag BPF_OK
-    else
-      upd_flag BPF_ILLEGAL_SHIFT
-  | op_BPF_RSH64i   => 
-    if complu_lt imm64 val64_64 then
-      do _ <- upd_reg dst (Val.shrlu   dst64 (sint32_to_vint imm));
-        upd_flag BPF_OK
-    else
-      upd_flag BPF_ILLEGAL_SHIFT
-  | op_BPF_NEG64    =>
-    do _ <- upd_reg dst (Val.negl    dst64);
-        upd_flag BPF_OK
-  | op_BPF_MOD64i   => 
-    if compl_ne imm64 val64_zero then
-      do _ <- upd_reg dst (val64_modlu dst64 (sint32_to_vint imm));
-        upd_flag BPF_OK
-    else
-      upd_flag BPF_ILLEGAL_DIV
-  | op_BPF_XOR64i   =>
-    do _ <- upd_reg dst (Val.xorl    dst64 imm64);
-        upd_flag BPF_OK
-  | op_BPF_MOV64i   =>
-    do _ <- upd_reg dst imm64;
-        upd_flag BPF_OK
-  | op_BPF_ARSH64i  => 
-    if complu_lt imm64 val64_64 then
-      do _ <- upd_reg dst (Val.shrl    dst64  (sint32_to_vint imm));
-        upd_flag BPF_OK
-    else
-      upd_flag BPF_ILLEGAL_SHIFT
-  | op_BPF_ALU64_IMM_ILLEGAL_INS => upd_flag BPF_ILLEGAL_INSTRUCTION
-  end.
+Definition comp_and_0x08_byte (x: int8_t): M bool :=  returnM (Byte.eq int8_zero (Byte.and x int8_0x08)).
 
-Definition step_opcode_alu64_reg (l: MyListType): M unit :=
-  do pc     <- eval_pc;
-  do ins    <- list_get l pc;
-  do dst    <- get_dst ins;
-  do dst64  <- eval_reg dst;
-  do src    <- get_src ins;
-  do src64  <- eval_reg src;
-  do opcode <- get_opcode_alu64_reg ins;
-  match opcode with
-  | op_BPF_ADD64r   => 
+(**r pc should be u32_t *)
+Definition step_opcode_alu64 (pc: int64_t) (dst: reg) (dst64: val64_t) (src64: val64_t) (op: int8_t): M unit :=
+  do opcode_alu64 <- get_opcode_alu64 op;
+  match opcode_alu64 with
+  | op_BPF_ADD64   => 
     do _ <- upd_reg dst (Val.addl    dst64 src64);
       upd_flag BPF_OK
-  | op_BPF_SUB64r   =>
+  | op_BPF_SUB64   =>
     do _ <- upd_reg dst (Val.subl    dst64 src64);
       upd_flag BPF_OK
-  | op_BPF_MUL64r   =>
+  | op_BPF_MUL64   =>
     do _ <- upd_reg dst (Val.mull    dst64 src64);
       upd_flag BPF_OK
-  | op_BPF_DIV64r   =>
+  | op_BPF_DIV64   =>
     if compl_ne src64 val64_zero then
       do _ <- upd_reg dst (val64_divlu dst64 src64);
         upd_flag BPF_OK
     else
       upd_flag BPF_ILLEGAL_DIV
-  | op_BPF_OR64r    =>
+  | op_BPF_OR64    =>
     do _ <- upd_reg dst (Val.orl     dst64 src64);
         upd_flag BPF_OK
-  | op_BPF_AND64r   =>
+  | op_BPF_AND64   =>
     do _ <- upd_reg dst (Val.andl    dst64 src64);
         upd_flag BPF_OK
-  | op_BPF_LSH64r   =>
+  | op_BPF_LSH64   =>
     do src32 <- reg64_to_reg32 src64;
     if complu_lt src64 val64_64 then
       do _ <- upd_reg dst (Val.shll    dst64 src32);
         upd_flag BPF_OK
     else
       upd_flag BPF_ILLEGAL_SHIFT
-  | op_BPF_RSH64r   =>
+  | op_BPF_RSH64   =>
     do src32 <- reg64_to_reg32 src64;
     if complu_lt src64 val64_64 then
       do _ <- upd_reg dst (Val.shrlu   dst64 src32);
         upd_flag BPF_OK
     else
       upd_flag BPF_ILLEGAL_SHIFT
-  | op_BPF_MOD64r   =>
+  | op_BPF_NEG64    =>
+    do _ <- upd_reg dst (Val.negl    dst64);
+        upd_flag BPF_OK
+  | op_BPF_MOD64   =>
     do src32 <- reg64_to_reg32 src64;
     if compl_ne src64 val64_zero then
       do _ <- upd_reg dst (val64_modlu dst64 src32);
         upd_flag BPF_OK
     else
       upd_flag BPF_ILLEGAL_DIV
-  | op_BPF_XOR64r   =>
+  | op_BPF_XOR64   =>
     do _ <- upd_reg dst (Val.xorl      dst64 src64);
         upd_flag BPF_OK
-  | op_BPF_MOV64r   =>
+  | op_BPF_MOV64   =>
     do _ <- upd_reg dst src64;
         upd_flag BPF_OK
-  | op_BPF_ARSH64r  =>
+  | op_BPF_ARSH64  =>
     do src32 <- reg64_to_reg32 src64;
     if complu_lt src64 val64_64 then
       do _ <- upd_reg dst (Val.shrl    dst64 src32);
         upd_flag BPF_OK
     else
       upd_flag BPF_ILLEGAL_SHIFT
-  | op_BPF_ALU64_REG_ILLEGAL_INS => upd_flag BPF_ILLEGAL_INSTRUCTION
+  | op_BPF_ALU64_ILLEGAL_INS => upd_flag BPF_ILLEGAL_INSTRUCTION
   end.
 
-Definition step_opcode_alu32_imm (l: MyListType): M unit :=
-  do pc     <- eval_pc;
-  do ins    <- list_get l pc;
-  do dst    <- get_dst ins;
-  do dst64  <- eval_reg dst;
-  do dst32  <- reg64_to_reg32 dst64;
-  do imm    <- get_immediate ins;
-  do opcode <- get_opcode_alu32_imm ins;
-  match opcode with
-  | op_BPF_ADD32i   =>
-    do _ <- upd_reg dst (Val.longofintu (Val.add dst32 (sint32_to_vint imm)));
+Definition step_opcode_alu32 (pc: int64_t) (dst: reg) (dst32: valu32_t) (src32: valu32_t) (op: int8_t): M unit :=
+  do opcode_alu32 <- get_opcode_alu32 op;
+  match opcode_alu32 with
+  | op_BPF_ADD32   =>
+    do _ <- upd_reg dst (Val.longofintu (Val.add dst32 src32));
         upd_flag BPF_OK
-  | op_BPF_SUB32i   =>
-    do _ <- upd_reg dst (Val.longofintu (Val.sub dst32 (sint32_to_vint imm)));
+  | op_BPF_SUB32   =>
+    do _ <- upd_reg dst (Val.longofintu (Val.sub dst32 src32));
         upd_flag BPF_OK
-  | op_BPF_MUL32i   =>
-    do _ <- upd_reg dst (Val.longofintu (Val.mul dst32 (sint32_to_vint imm)));
+  | op_BPF_MUL32   =>
+    do _ <- upd_reg dst (Val.longofintu (Val.mul dst32 src32));
         upd_flag BPF_OK
-  | op_BPF_DIV32i   =>
-    if compl_ne_32 (sint32_to_vint imm) Vzero then
-      do _ <- upd_reg dst (Val.longofintu (val32_divu dst32 (sint32_to_vint imm)));
+  | op_BPF_DIV32   =>
+    if compl_ne_32 src32 Vzero then
+      do _ <- upd_reg dst (Val.longofintu (val32_divu dst32 src32));
         upd_flag BPF_OK
     else
       upd_flag BPF_ILLEGAL_DIV
-  | op_BPF_OR32i   =>
-    do _ <- upd_reg dst (Val.longofintu (Val.or  dst32 (sint32_to_vint imm)));
+  | op_BPF_OR32   =>
+    do _ <- upd_reg dst (Val.longofintu (Val.or  dst32 src32));
         upd_flag BPF_OK
-  | op_BPF_AND32i   =>
-    do _ <- upd_reg dst (Val.longofintu (Val.and dst32 (sint32_to_vint imm)));
+  | op_BPF_AND32   =>
+    do _ <- upd_reg dst (Val.longofintu (Val.and dst32 src32));
         upd_flag BPF_OK
-  | op_BPF_LSH32i   =>
-    if complu_lt_32 (sint32_to_vint imm) val32_32 then (**r Int.iwordsize = int32_32 *)
-      do _ <- upd_reg dst (Val.longofintu (Val.shl dst32 (sint32_to_vint imm)));
+  | op_BPF_LSH32   =>
+    if complu_lt_32 src32 val32_32 then
+      do _ <- upd_reg dst (Val.longofintu (Val.shl dst32 src32));
         upd_flag BPF_OK
     else
       upd_flag BPF_ILLEGAL_SHIFT
-  | op_BPF_RSH32i   =>
-    if complu_lt_32 (sint32_to_vint imm) val32_32 then
-      do _ <- upd_reg dst (Val.longofintu (Val.shru dst32 (sint32_to_vint imm)));
+  | op_BPF_RSH32   =>
+    if complu_lt_32 src32 val32_32 then
+      do _ <- upd_reg dst (Val.longofintu (Val.shru dst32 src32));
         upd_flag BPF_OK
     else
       upd_flag BPF_ILLEGAL_SHIFT
   | op_BPF_NEG32    =>
     do _ <- upd_reg dst (Val.longofintu (Val.neg dst32));
         upd_flag BPF_OK
-  | op_BPF_MOD32i   =>
-    if compl_ne_32 (sint32_to_vint imm) Vzero then
-      do _ <- upd_reg dst (Val.longofintu (val32_modu dst32 (sint32_to_vint imm)));
-        upd_flag BPF_OK
-    else
-      upd_flag BPF_ILLEGAL_DIV
-  | op_BPF_XOR32i   =>
-    do _ <- upd_reg dst (Val.longofintu (Val.xor dst32 (sint32_to_vint imm)));
-        upd_flag BPF_OK
-  | op_BPF_MOV32i   =>
-    do _ <- upd_reg dst (sint32_to_vint imm);
-        upd_flag BPF_OK
-  | op_BPF_ARSH32i  =>
-    if complu_lt_32 (sint32_to_vint imm) val32_32 then
-      do _ <- upd_reg dst (Val.longofintu (Val.shr dst32 (sint32_to_vint imm)));
-        upd_flag BPF_OK
-    else
-      upd_flag BPF_ILLEGAL_SHIFT
-  | op_BPF_ALU32_IMM_ILLEGAL_INS => upd_flag BPF_ILLEGAL_INSTRUCTION
-  end.
-
-
-Definition step_opcode_alu32_reg (l: MyListType): M unit :=
-  do pc     <- eval_pc;
-  do ins    <- list_get l pc;
-  do dst    <- get_dst ins;
-  do dst64  <- eval_reg dst;
-  do dst32  <- reg64_to_reg32 dst64;
-  do src    <- get_src ins;
-  do src64  <- eval_reg src;
-  do src32  <- reg64_to_reg32 src64;
-  do opcode <- get_opcode_alu32_reg ins;
-  match opcode with
-  | op_BPF_ADD32r   =>
-    do _ <- upd_reg dst (Val.longofintu (Val.add dst32 src32));
-        upd_flag BPF_OK
-  | op_BPF_SUB32r   =>
-    do _ <- upd_reg dst (Val.longofintu (Val.sub dst32 src32));
-        upd_flag BPF_OK
-  | op_BPF_MUL32r   =>
-    do _ <- upd_reg dst (Val.longofintu (Val.mul dst32 src32));
-        upd_flag BPF_OK
-  | op_BPF_DIV32r   =>
-    if compl_ne_32 src32 Vzero then
-      do _ <- upd_reg dst (Val.longofintu (val32_divu dst32 src32));
-        upd_flag BPF_OK
-    else
-      upd_flag BPF_ILLEGAL_DIV
-  | op_BPF_OR32r   =>
-    do _ <- upd_reg dst (Val.longofintu (Val.or  dst32 src32));
-        upd_flag BPF_OK
-  | op_BPF_AND32r   =>
-    do _ <- upd_reg dst (Val.longofintu (Val.and dst32 src32));
-        upd_flag BPF_OK
-  | op_BPF_LSH32r   =>
-    if complu_lt_32 src32 val32_32 then
-      do _ <- upd_reg dst (Val.longofintu (Val.shl dst32 src32));
-        upd_flag BPF_OK
-    else
-      upd_flag BPF_ILLEGAL_SHIFT
-  | op_BPF_RSH32r   =>
-    if complu_lt_32 src32 val32_32 then
-      do _ <- upd_reg dst (Val.longofintu (Val.shru dst32 src32));
-        upd_flag BPF_OK
-    else
-      upd_flag BPF_ILLEGAL_SHIFT
-  | op_BPF_MOD32r   =>
+  | op_BPF_MOD32   =>
     if compl_ne_32 src32 Vzero then
       do _ <- upd_reg dst (Val.longofintu (val32_modu dst32 src32));
         upd_flag BPF_OK
     else
       upd_flag BPF_ILLEGAL_DIV
-  | op_BPF_XOR32r   =>
+  | op_BPF_XOR32   =>
     do _ <- upd_reg dst (Val.longofintu (Val.xor dst32 src32));
         upd_flag BPF_OK
-  | op_BPF_MOV32r   =>
+  | op_BPF_MOV32   =>
     do _ <- upd_reg dst src32;
         upd_flag BPF_OK
-  | op_BPF_ARSH32r  =>
+  | op_BPF_ARSH32  =>
     if complu_lt_32 src32 val32_32 then
       do _ <- upd_reg dst (Val.longofintu (Val.shr dst32 src32));
         upd_flag BPF_OK
     else
       upd_flag BPF_ILLEGAL_SHIFT
-  | op_BPF_ALU32_REG_ILLEGAL_INS => upd_flag BPF_ILLEGAL_INSTRUCTION
+  | op_BPF_ALU32_ILLEGAL_INS => upd_flag BPF_ILLEGAL_INSTRUCTION
   end.
 
-Definition step_opcode_branch_imm (l: MyListType): M unit :=
-  do pc     <- eval_pc;
-  do ins    <- list_get l pc;
-  do dst    <- get_dst ins;
-  do dst64  <- eval_reg dst;
-  do ofs    <- get_offset ins;
-  do imm    <- get_immediate ins;
-  do opcode <- get_opcode_branch_imm ins;
-  match opcode with
+(**r ofs should be sint16_t *)
+Definition step_opcode_branch (pc: int64_t) (dst64: val64_t) (src64: val64_t) (op: int8_t) (ofs: int64_t): M unit :=
+  do opcode_jmp <- get_opcode_branch op;
+  match opcode_jmp with
   | op_BPF_JA       =>
      do _ <- upd_pc (Int64.add pc ofs);
         upd_flag BPF_OK
-  | op_BPF_JEQi     =>
-    if compl_eq dst64 (Val.longofintu (sint32_to_vint imm)) then
-      do _ <- upd_pc (Int64.add pc ofs);
-        upd_flag BPF_OK
-    else
-      upd_flag BPF_OK
-  | op_BPF_JGTi     =>
-    if complu_gt dst64 (Val.longofintu (sint32_to_vint imm)) then
-      do _ <- upd_pc (Int64.add pc ofs);
-        upd_flag BPF_OK
-    else
-      upd_flag BPF_OK
-  | op_BPF_JGEi     =>
-    if complu_ge dst64 (Val.longofintu (sint32_to_vint imm)) then
-      do _ <- upd_pc (Int64.add pc ofs);
-        upd_flag BPF_OK
-    else
-      upd_flag BPF_OK
-  | op_BPF_JLTi     =>
-    if complu_lt dst64 (Val.longofintu (sint32_to_vint imm)) then
-      do _ <- upd_pc (Int64.add pc ofs);
-        upd_flag BPF_OK
-    else
-      upd_flag BPF_OK
-  | op_BPF_JLEi     =>
-    if complu_le dst64 (Val.longofintu (sint32_to_vint imm)) then
-      do _ <- upd_pc (Int64.add pc ofs);
-        upd_flag BPF_OK
-    else
-      upd_flag BPF_OK
-  | op_BPF_JSETi     =>
-    if complu_set dst64 (Val.longofintu (sint32_to_vint imm)) then
-      do _ <- upd_pc (Int64.add pc ofs);
-        upd_flag BPF_OK
-    else
-      upd_flag BPF_OK
-  | op_BPF_JNEi     =>
-    if compl_ne dst64 (Val.longofintu (sint32_to_vint imm)) then
-      do _ <- upd_pc (Int64.add pc ofs);
-        upd_flag BPF_OK
-    else
-      upd_flag BPF_OK
-  | op_BPF_JSGTi     =>
-    if compl_gt dst64 (Val.longofintu (sint32_to_vint imm)) then
-      do _ <- upd_pc (Int64.add pc ofs);
-        upd_flag BPF_OK
-    else
-      upd_flag BPF_OK
-  | op_BPF_JSGEi     =>
-    if compl_ge dst64 (Val.longofintu (sint32_to_vint imm)) then
-      do _ <- upd_pc (Int64.add pc ofs);
-        upd_flag BPF_OK
-    else
-      upd_flag BPF_OK
-  | op_BPF_JSLTi     =>
-    if compl_lt dst64 (Val.longofintu (sint32_to_vint imm)) then
-      do _ <- upd_pc (Int64.add pc ofs);
-        upd_flag BPF_OK
-    else
-      upd_flag BPF_OK
-  | op_BPF_JSLEi     =>
-    if compl_le dst64 (Val.longofintu (sint32_to_vint imm)) then
-      do _ <- upd_pc (Int64.add pc ofs);
-        upd_flag BPF_OK
-    else
-      upd_flag BPF_OK
-  | op_BPF_RET => upd_flag BPF_SUCC_RETURN
-  | op_BPF_JMP_IMM_ILLEGAL_INS => upd_flag BPF_ILLEGAL_INSTRUCTION
-  end.
 
-Definition step_opcode_branch_reg (l: MyListType): M unit :=
-  do pc     <- eval_pc;
-  do ins    <- list_get l pc;
-  do dst    <- get_dst ins;
-  do dst64  <- eval_reg dst;
-  do src    <- get_src ins;
-  do src64  <- eval_reg src;
-  do ofs    <- get_offset ins;
-  do opcode <- get_opcode_branch_reg ins;
-  match opcode with
-  | op_BPF_JEQr     =>
+  | op_BPF_JEQ     =>
     if compl_eq dst64 src64 then
       do _ <- upd_pc (Int64.add pc ofs);
         upd_flag BPF_OK
     else
       upd_flag BPF_OK
-  | op_BPF_JGTr     =>
+  | op_BPF_JGT     =>
     if complu_gt dst64 src64 then
       do _ <- upd_pc (Int64.add pc ofs);
         upd_flag BPF_OK
     else
       upd_flag BPF_OK
-  | op_BPF_JGEr     =>
+  | op_BPF_JGE     =>
     if complu_ge dst64 src64 then
       do _ <- upd_pc (Int64.add pc ofs);
         upd_flag BPF_OK
     else
       upd_flag BPF_OK
-  | op_BPF_JLTr     =>
+  | op_BPF_JLT     =>
     if complu_lt dst64 src64 then
       do _ <- upd_pc (Int64.add pc ofs);
         upd_flag BPF_OK
     else
       upd_flag BPF_OK
-  | op_BPF_JLEr     =>
+  | op_BPF_JLE     =>
     if complu_le dst64 src64 then
       do _ <- upd_pc (Int64.add pc ofs);
         upd_flag BPF_OK
     else
       upd_flag BPF_OK
-  | op_BPF_JSETr     =>
+  | op_BPF_JSET     =>
     if complu_set dst64 src64 then
       do _ <- upd_pc (Int64.add pc ofs);
         upd_flag BPF_OK
     else
       upd_flag BPF_OK
-  | op_BPF_JNEr     =>
+  | op_BPF_JNE     =>
     if compl_ne dst64 src64 then
       do _ <- upd_pc (Int64.add pc ofs);
         upd_flag BPF_OK
     else
       upd_flag BPF_OK
-  | op_BPF_JSGTr     =>
+  | op_BPF_JSGT     =>
     if compl_gt dst64 src64 then
       do _ <- upd_pc (Int64.add pc ofs);
         upd_flag BPF_OK
     else
       upd_flag BPF_OK
-  | op_BPF_JSGEr     =>
+  | op_BPF_JSGE     =>
     if compl_ge dst64 src64 then
       do _ <- upd_pc (Int64.add pc ofs);
         upd_flag BPF_OK
     else
       upd_flag BPF_OK
-  | op_BPF_JSLTr     =>
+  | op_BPF_JSLT     =>
     if compl_lt dst64 src64 then
       do _ <- upd_pc (Int64.add pc ofs);
         upd_flag BPF_OK
     else
       upd_flag BPF_OK
-  | op_BPF_JSLEr     =>
+  | op_BPF_JSLE     =>
     if compl_le dst64 src64 then
       do _ <- upd_pc (Int64.add pc ofs);
         upd_flag BPF_OK
     else
       upd_flag BPF_OK
-  | op_BPF_JMP_REG_ILLEGAL_INS => upd_flag BPF_ILLEGAL_INSTRUCTION
+
+  | op_BPF_RET => upd_flag BPF_SUCC_RETURN
+  | op_BPF_JMP_ILLEGAL_INS => upd_flag BPF_ILLEGAL_INSTRUCTION
   end.
 
-Definition step_opcode_mem_ld_imm (l: MyListType) (len: int64_t): M unit :=
-  do pc     <- eval_pc;
-  do ins    <- list_get l pc;
-  do dst    <- get_dst ins;
-  do dst64  <- eval_reg dst;
-  do ofs    <- get_offset ins;
-  do imm    <- get_immediate ins;
-  do imm64  <- eval_immediate imm;
-  do opcode <- get_opcode_mem_ld_imm ins;
-  match opcode with
+Definition step_opcode_mem_ld_imm (pc: int64_t) (dst: reg) (dst64: val64_t) (imm64: val64_t) (op: int8_t) (len: int64_t) (l: MyListType): M unit :=
+  do opcode_ld <- get_opcode_mem_ld_imm op;
+  match opcode_ld with
   | op_BPF_LDDW      =>
     if (Int64.ltu (Int64.add pc Int64.one) len) then (**r pc+1 < len: pc+1 is less than the length of l *)
       do next_ins <- list_get l (Int64.add pc Int64.one);
@@ -618,19 +385,11 @@ Definition step_opcode_mem_ld_imm (l: MyListType) (len: int64_t): M unit :=
   | op_BPF_LDX_IMM_ILLEGAL_INS => upd_flag BPF_ILLEGAL_INSTRUCTION
   end.
 
-Definition step_opcode_mem_ld_reg (l: MyListType): M unit :=
-  do pc     <- eval_pc;
-  do ins    <- list_get l pc;
-  do dst    <- get_dst ins;
-  do src    <- get_src ins;
-  do src64  <- eval_reg src;
-  do ofs    <- get_offset ins;
-  do ofs64  <- eval_offset ofs;
-  do opcode <- get_opcode_mem_ld_reg ins;
-  do addr_src <- get_addl src64 ofs64;
-  match opcode with
+Definition step_opcode_mem_ld_reg (pc: int64_t) (dst: reg) (dst64: val64_t) (src64: val64_t) (op: int8_t) (ofs64: val64_t) (addr: val64_t) (l: MyListType): M unit :=
+  do opcode_ld <- get_opcode_mem_ld_reg op;
+  match opcode_ld with
   | op_BPF_LDXW      =>
-    do check_ldxw <- check_mem l addr_src Mint32;
+    do check_ldxw <- check_mem l addr Mint32;
       if compl_eq check_ldxw val64_zero then
         upd_flag BPF_ILLEGAL_MEM
       else
@@ -638,7 +397,7 @@ Definition step_opcode_mem_ld_reg (l: MyListType): M unit :=
         do _ <- upd_reg dst v_xw;
           upd_flag BPF_OK
   | op_BPF_LDXH      =>
-    do check_ldxh <- check_mem l addr_src Mint16unsigned;
+    do check_ldxh <- check_mem l addr Mint16unsigned;
       if compl_eq check_ldxh val64_zero then
         upd_flag BPF_ILLEGAL_MEM
       else
@@ -646,7 +405,7 @@ Definition step_opcode_mem_ld_reg (l: MyListType): M unit :=
         do _ <- upd_reg dst v_xh;
           upd_flag BPF_OK
   | op_BPF_LDXB      =>
-    do check_ldxb <- check_mem l addr_src Mint8unsigned;
+    do check_ldxb <- check_mem l addr Mint8unsigned;
       if compl_eq check_ldxb val64_zero then
         upd_flag BPF_ILLEGAL_MEM
       else
@@ -654,7 +413,7 @@ Definition step_opcode_mem_ld_reg (l: MyListType): M unit :=
         do _ <- upd_reg dst v_xb;
           upd_flag BPF_OK
   | op_BPF_LDXDW     =>
-    do check_ldxdw <- check_mem l addr_src Mint64;
+    do check_ldxdw <- check_mem l addr Mint64;
       if compl_eq check_ldxdw val64_zero then
         upd_flag BPF_ILLEGAL_MEM
       else
@@ -664,83 +423,66 @@ Definition step_opcode_mem_ld_reg (l: MyListType): M unit :=
   | op_BPF_LDX_REG_ILLEGAL_INS => upd_flag BPF_ILLEGAL_INSTRUCTION
   end.
 
-Definition step_opcode_mem_st_imm (l: MyListType): M unit :=
-  do pc     <- eval_pc;
-  do ins    <- list_get l pc;
-  do dst    <- get_dst ins;
-  do dst64  <- eval_reg dst;
-  do ofs    <- get_offset ins;
-  do ofs64  <- eval_offset ofs;
-  do imm    <- get_immediate ins;
-  do addr_dst <- get_addl dst64 ofs64;
-  do opcode <- get_opcode_mem_st_imm ins;
-  match opcode with
+Definition step_opcode_mem_st_imm (pc: int64_t) (dst: reg) (dst64: val64_t) (imm: vals32_t) (op: int8_t) (ofs64: val64_t) (addr: val64_t) (l: MyListType): M unit :=
+  do opcode_st <- get_opcode_mem_st_imm op;
+  match opcode_st with
   | op_BPF_STW       =>
-    do check_stw <- check_mem l addr_dst Mint32;
+    do check_stw <- check_mem l addr Mint32;
       if compl_eq check_stw val64_zero then
         upd_flag BPF_ILLEGAL_MEM
       else
-        do _ <- store_mem_imm Mint32 (Val.addl dst64 ofs64) (sint32_to_vint imm);
+        do _ <- store_mem_imm Mint32 (Val.addl dst64 ofs64) imm;
           upd_flag BPF_OK
   | op_BPF_STH       =>
-    do check_sth <- check_mem l addr_dst Mint16unsigned;
+    do check_sth <- check_mem l addr Mint16unsigned;
       if compl_eq check_sth val64_zero then
         upd_flag BPF_ILLEGAL_MEM
       else
-        do _ <- store_mem_imm Mint16unsigned (Val.addl dst64 ofs64) (sint32_to_vint imm);
+        do _ <- store_mem_imm Mint16unsigned (Val.addl dst64 ofs64) imm;
           upd_flag BPF_OK
   | op_BPF_STB       =>
-    do check_stb <- check_mem l addr_dst Mint8unsigned;
+    do check_stb <- check_mem l addr Mint8unsigned;
       if compl_eq check_stb val64_zero then
         upd_flag BPF_ILLEGAL_MEM
       else
-        do _ <- store_mem_imm Mint8unsigned (Val.addl dst64 ofs64) (sint32_to_vint imm);
+        do _ <- store_mem_imm Mint8unsigned (Val.addl dst64 ofs64) imm;
           upd_flag BPF_OK
   | op_BPF_STDW      =>
-    do check_stdw <- check_mem l addr_dst Mint64;
+    do check_stdw <- check_mem l addr Mint64;
       if compl_eq check_stdw val64_zero then
         upd_flag BPF_ILLEGAL_MEM
       else
-        do _ <- store_mem_imm Mint64 (Val.addl dst64 ofs64) (sint32_to_vint imm);
+        do _ <- store_mem_imm Mint64 (Val.addl dst64 ofs64) imm;
           upd_flag BPF_OK
   | op_BPF_ST_IMM_ILLEGAL_INS => upd_flag BPF_ILLEGAL_INSTRUCTION
   end.
 
-Definition step_opcode_mem_st_reg (l: MyListType): M unit :=
-  do pc     <- eval_pc;
-  do ins    <- list_get l pc;
-  do dst    <- get_dst ins;
-  do dst64  <- eval_reg dst;
-  do src    <- get_src ins;
-  do src64  <- eval_reg src;
-  do ofs    <- get_offset ins;
-  do ofs64  <- eval_offset ofs;
-  do addr_dst <- get_addl dst64 ofs64;
-  do opcode <- get_opcode_mem_st_reg ins;
-  match opcode with
+Definition step_opcode_mem_st_reg (pc: int64_t) (dst: reg) (dst64: val64_t) (src64: val64_t) (op: int8_t) (ofs64: val64_t) (addr: val64_t) (l: MyListType): M unit :=
+  do opcode_st <- get_opcode_mem_st_reg op;
+  match opcode_st with
   | op_BPF_STXW      =>
-    do check_stxw <- check_mem l addr_dst Mint32;
+    do check_stxw <- check_mem l addr Mint32;
       if compl_eq check_stxw val64_zero then
         upd_flag BPF_ILLEGAL_MEM
       else
         do _ <- store_mem_reg Mint32 (Val.addl dst64 ofs64) src64;
           upd_flag BPF_OK
   | op_BPF_STXH      =>
-    do check_stxh <- check_mem l addr_dst Mint16unsigned;
+    do check_stxh <- check_mem l addr Mint16unsigned;
       if compl_eq check_stxh val64_zero then
         upd_flag BPF_ILLEGAL_MEM
       else
         do _ <- store_mem_reg Mint16unsigned (Val.addl dst64 ofs64) src64;
           upd_flag BPF_OK
   | op_BPF_STXB      =>
-    do check_stxb <- check_mem l addr_dst Mint8unsigned;
+    do check_stxb <- check_mem l addr Mint8unsigned;
       if compl_eq check_stxb val64_zero then
         upd_flag BPF_ILLEGAL_MEM
       else
         do _ <- store_mem_reg Mint8unsigned (Val.addl dst64 ofs64) src64;
           upd_flag BPF_OK
   | op_BPF_STXDW     =>
-    do check_stxdw <- check_mem l addr_dst Mint64;
+    do check_stxdw <- check_mem l addr Mint64;
       if compl_eq check_stxdw val64_zero then
         upd_flag BPF_ILLEGAL_MEM
       else
@@ -749,46 +491,109 @@ Definition step_opcode_mem_st_reg (l: MyListType): M unit :=
   | op_BPF_STX_REG_ILLEGAL_INS => upd_flag BPF_ILLEGAL_INSTRUCTION
   end.
 
-Definition step (l: MyListType) (len: int64_t): M unit :=
-  do pc <- eval_pc;
-  do ins <- list_get l pc;
-  do op <- get_opcode ins;
-  match op with
-  | op_BPF_ALU64_imm   => step_opcode_alu64_imm l       (**r 0xX7 *)
-  | op_BPF_ALU64_reg   => step_opcode_alu64_reg l       (**r 0xXf *)
-  | op_BPF_ALU32_imm   => step_opcode_alu32_imm l       (**r 0xX4 *)
-  | op_BPF_ALU32_reg   => step_opcode_alu32_reg l       (**r 0xXc *)
-  | op_BPF_Branch_imm  => step_opcode_branch_imm l      (**r 0xX5 *)
-  | op_BPF_Branch_reg  => step_opcode_branch_reg l      (**r 0xXd *)
-  | op_BPF_Mem_ld_imm  => step_opcode_mem_ld_imm l len  (**r 0xX8 *)
-  | op_BPF_Mem_ld_reg  => step_opcode_mem_ld_reg l      (**r 0xX1/0xX9 *)
-  | op_BPF_Mem_st_imm  => step_opcode_mem_st_imm l      (**r 0xX2/0xXa *)
-  | op_BPF_Mem_st_reg  => step_opcode_mem_st_reg l      (**r 0xX3/0xXb *)
-
+Definition step (len: int64_t) (l: MyListType): M unit :=
+  do pc   <- eval_pc;
+  do ins  <- list_get l pc;
+  do op   <- get_opcode_ins ins;
+  do opc  <- get_opcode op;
+  match opc with
+  | op_BPF_ALU64   =>
+    do dst    <- get_dst ins;
+    do dst64  <- eval_reg dst;
+      (**r #define BPF_INSTRUCTION_ALU_S_MASK      0x08 *)
+    do is_imm <- comp_and_0x08_byte op;
+      if is_imm then
+        do imm    <- get_immediate ins;
+        do imm64  <- eval_immediate imm;
+        step_opcode_alu64 pc dst dst64 imm64 op
+      else
+        do src    <- get_src ins;
+        do src64  <- eval_reg src;
+        step_opcode_alu64 pc dst dst64 src64 op                     (**r 0xX7 / 0xXf *)
+  | op_BPF_ALU32   =>
+    do dst    <- get_dst ins;
+    do dst64  <- eval_reg dst;
+    do dst32  <- reg64_to_reg32 dst64;
+      (**r #define BPF_INSTRUCTION_ALU_S_MASK      0x08 *)
+    do is_imm <- comp_and_0x08_byte op;
+      if is_imm then
+        do imm    <- get_immediate ins;
+        step_opcode_alu32 pc dst dst32 (sint32_to_vint imm) op
+      else
+        do src    <- get_src ins;
+        do src64  <- eval_reg src;
+        do src32  <- reg64_to_reg32 src64;
+        step_opcode_alu32 pc dst dst32 src32 op                     (**r 0xX4 / 0xXc *)
+  | op_BPF_Branch  =>
+    do dst    <- get_dst ins;
+    do dst64  <- eval_reg dst;
+    do ofs    <- get_offset ins;
+      (**r #define BPF_INSTRUCTION_ALU_S_MASK      0x08 *)
+    do is_imm <- comp_and_0x08_byte op;
+      if is_imm then
+        do imm    <- get_immediate ins;
+        do imm64  <- eval_immediate imm;
+        step_opcode_branch pc dst64 imm64 op ofs
+      else
+        do src    <- get_src ins;
+        do src64  <- eval_reg src;
+        step_opcode_branch pc dst64 src64 op ofs                    (**r 0xX5 / 0xXd *)
+  | op_BPF_Mem_ld_imm  =>
+    do dst    <- get_dst ins;
+    do dst64  <- eval_reg dst;
+    do imm    <- get_immediate ins;
+    do imm64  <- eval_immediate imm;
+    step_opcode_mem_ld_imm pc dst dst64 imm64 op len l              (**r 0xX8 *)
+  | op_BPF_Mem_ld_reg  =>
+    do dst    <- get_dst ins;
+    do dst64  <- eval_reg dst;
+    do src    <- get_src ins;
+    do src64  <- eval_reg src;
+    do ofs    <- get_offset ins;
+    do ofs64  <- eval_offset ofs;
+    do addr   <- get_addl src64 ofs64;
+    step_opcode_mem_ld_reg pc dst dst64 src64 op ofs64 addr l       (**r 0xX1/0xX9 *)
+  | op_BPF_Mem_st_imm  =>
+    do dst    <- get_dst ins;
+    do dst64  <- eval_reg dst;
+    do ofs    <- get_offset ins;
+    do ofs64  <- eval_offset ofs;
+    do imm    <- get_immediate ins;
+    do addr   <- get_addl dst64 ofs64;
+    step_opcode_mem_st_imm pc dst dst64 (sint32_to_vint imm) op ofs64 addr l      (**r 0xX2/0xXa *)
+  | op_BPF_Mem_st_reg  =>
+    do dst    <- get_dst ins;
+    do dst64  <- eval_reg dst;
+    do src    <- get_src ins;
+    do src64  <- eval_reg src;
+    do ofs    <- get_offset ins;
+    do ofs64  <- eval_offset ofs;
+    do addr <- get_addl dst64 ofs64;
+    step_opcode_mem_st_reg pc dst dst64 src64 op ofs64 addr l      (**r 0xX3/0xXb *)
   | op_BPF_ILLEGAL_INS => upd_flag BPF_ILLEGAL_INSTRUCTION
   end.
 
-Fixpoint bpf_interpreter_aux (l: MyListType) (len: int64_t) (fuel: nat) {struct fuel}: M unit :=
+Fixpoint bpf_interpreter_aux (len: int64_t) (fuel: nat) (l: MyListType) {struct fuel}: M unit :=
   match fuel with
   | O => upd_flag BPF_ILLEGAL_LEN
   | S fuel =>
     do pc <- eval_pc;
       if Int64.ltu pc len then (**r pc < len: pc is less than the length of l *)
-        do _ <- step l len;
+        do _ <- step len l;
         do _ <- upd_pc_incr;
         do f <- eval_flag;
           if flag_eq f BPF_OK then
-            bpf_interpreter_aux l len fuel
+            bpf_interpreter_aux len fuel l
           else
             returnM tt
       else
         upd_flag BPF_ILLEGAL_LEN
   end.
 
-Definition bpf_interpreter (l: MyListType) (len: int64_t) (fuel: nat): M val64_t :=
+Definition bpf_interpreter (len: int64_t) (fuel: nat) (l: MyListType): M val64_t :=
   do mrs<- eval_mem_regions;
   do _  <- upd_reg R1 (start_addr (bpf_ctx mrs));
-  do _  <- bpf_interpreter_aux l len fuel;
+  do _  <- bpf_interpreter_aux len fuel l;
   do f <- eval_flag;
     if flag_eq f BPF_SUCC_RETURN then
       eval_reg R0
