tests/Tests.v
@@ -48,12 +48,10 @@ GenerateIntermediateRepresentation SymbolIRs
   eval_offset
   get_immediate
   eval_immediate
-  get_opcode_alu64_imm
-  get_opcode_alu64_reg
-  get_opcode_alu32_imm
-  get_opcode_alu32_reg
-  get_opcode_branch_imm
-  get_opcode_branch_reg
+  get_opcode_ins
+  get_opcode_alu64
+  get_opcode_alu32
+  get_opcode_branch
   get_opcode_mem_ld_imm
   get_opcode_mem_ld_reg
   get_opcode_mem_st_imm
@@ -67,12 +65,10 @@ GenerateIntermediateRepresentation SymbolIRs
   is_well_chunk_bool
   check_mem_aux
   check_mem
-  step_opcode_alu64_imm
-  step_opcode_alu64_reg
-  step_opcode_alu32_imm
-  step_opcode_alu32_reg
-  step_opcode_branch_imm
-  step_opcode_branch_reg
+  comp_and_0x08_byte
+  step_opcode_alu64
+  step_opcode_alu32
+  step_opcode_branch
   step_opcode_mem_ld_imm
   step_opcode_mem_ld_reg
   step_opcode_mem_st_imm
